% TODO
% \FloatInTheorem

% \begin{proof}~

% \begin{tabbing}

% \end{tabbing}
% \end{proof}

The let floating transformations move lazy let constructs, in and out of other
constructs, to further unblock more optimisations.
%
In essence, since let bindings consume resources lazily (by introducing a
$\D$-variable with usage environment $\D$, where $\D$ is the typing environment
of the bound expression), we can intuitively move them around without violating linearity.
%
We prove let floating transformations \emph{full-laziness} and three
\emph{local-transformations} preserve types and linearity.

\FullLazinessTheorem

\begin{proof}~

\begin{tabbing}
    (1) $\G; \D,\D' \vdash \lambda \y[\pi].~\llet{\xD = e}{e'} : \s' \to \vp$\\
    Subcase $\pi = 1$\\
    (2) $\G; \D,\D',\y[1] \vdash \llet{\xD = e}{e'} : \vp$\`by inv. on $\lambda I$\\
    (3) $\G; \D \vdash e : \s$\` by inv. on (let)\\
    (4) $\G, \xD; \D, \D', \y[1] \vdash e' : \vp$\`by inv. on (let)\\
    (5) $\G, \xD; \D, \D' \vdash \lambda \y[1].~e' : \s' \to \vp$\`by ($\lambda I$) (4)\\
    (6) $\G; \D,\D' \vdash \llet{\xD = e}{\lambda \y[1].~e'} : \s' \to \vp$ by (let) $(3,5)$\\
    Subcase $\pi = \omega$\\
    As above but $x$ is put in the unrestricted context $\G$
\end{tabbing}
\end{proof}


\LocalTransformationsTheorem

\begin{description}
\item[1.] Commuting Let-app
\begin{proof}~
\begin{tabbing}
    (1) $\G; \D, \D', \D'' \vdash (\llet{\xD = e_1}{e_2})~e_3 : \vp$\\
    (2) $\G; \D, \D' \vdash \llet{\xD = e_1}{e_2} : \s' \to_\pi \vp$ \`by inv. on 1\\
    (3) $\G; \D'' \vdash e_3 : \s'$\`by inv. on 1\\
    (4) $\G; \D \vdash e_1 : \s$\`by inv. on 2\\
    (5) $\G, \xD; \D, \D' \vdash e_2 : \s' \to_\pi \vp$\`by inv. on 2\\
    (6) $\G, \xD; \D, \D', \D'' \vdash e_2~e_3 : \vp$\` by $\lambda_\pi E$\\
    (7) $\G; \D, \D', \D'' \vdash \llet{\xD = e_1}{e_2~e_3} : \vp$\`by let (4,6)\\
\end{tabbing}
\end{proof}

\item[2.] Commuting let-case
\begin{proof}~
\begin{tabbing}
    (1) $\G; \D, \D', \D'' \vdash \ccase{\llet{\xD = e_1}{e_2}}{\z[\D,\D'][\s']~\{\ov{\rho \Rightarrow e_3}\}} : \vp$\\
    (2) $\G; \D, \D' \vdash \llet{\xD = e_1}{e_2} : \s'$\`by inv. on 1\\
    (3) $\G; \D \vdash e_1 : \s$\`by inv. on 2\\
    (4) $\G, \xD;\D,\D' \vdash e_2 : \s'$\`by inv. on 2\\
    Subcase $e_2$ is in WHNF\\
    (5) $\ov{\G,\z[\D,\D'][\s']; \D, \D', \D'' \vdash_{alt} \rho \Rightarrow e_3 :^z_{\D,\D'} \s' \Mapsto \vp}$\`by inv. on 1\\
    (6) $\G, \xD; \D, \D', \D'' \vdash \ccase{e_2}{\z[\D,\D'][\s']~\{\ov{\rho \Rightarrow e_3}\}} : \vp$\`by CaseWHNF (4,5)\\
    (7) $\G; \D, \D', \D'' \vdash \llet{\xD = e_1}{\ccase{e_2}{\z[\D,\D'][\s']~\{\ov{\rho \Rightarrow e_3}\}}} : \vp$\`by Let (3,6)\\
    Subcase $e_2$ is not in WHNF\\
    (5) $\ov{\G,\z[\irr{\D,\D'}][\s']; \irr{\D, \D'}, \D'' \vdash_{alt} \rho \Rightarrow e_3 :^z_{\irr{\D,\D'}} \s' \Rrightarrow \vp}$\`by inv. on 1\\
    (6) $\G, \xD; \D, \D', \D'' \vdash \ccase{e_2}{\z[\D,\D'][\s']~\{\ov{\rho \Rightarrow e_3}\}} : \vp$\`by CaseWHNF (4,5)\\
    (7) $\G; \D, \D', \D'' \vdash \llet{\xD = e_1}{\ccase{e_2}{\z[\D,\D'][\s']~\{\ov{\rho \Rightarrow e_3}\}}} : \vp$\`by Let (3,6)\\
\end{tabbing}
\end{proof}

\item[3.] Commuting let-let
\begin{proof}~
\begin{tabbing}
    (1) $\G, \D;\D',\D'' \vdash \llet{\x[\D,\D'][\s'] = (\llet{\yD = e_1}{e_2})}{e_3} : \vp$\\
    (2) $\G; \D, \D' \vdash \llet{\yD = e_1}{e_2} : \s'$\`by inv. on 1\\
    (3) $\G, \x[\D,\D'][\s'];\D,\D',\D'' \vdash e_3$\`by inv. on 1\\
    (4) $\G; \D \vdash e_1 : \s$\`by inv. on 2\\
    (5) $\G, \yD; \D,\D' \vdash e_2 : \s'$\`by inv. on 2\\
    (6) $\G, \yD; \D,\D',\D'' \vdash \llet{\x[\D,\D'][\s'] = e_2}{e_3} : \vp$\`by Let (3,5) and Weaken\\
    (7) $\G; \D,\D',\D'' \vdash \llet{\yD = e_1}{\llet{\x[\D,\D'][\s'] = e_2}{e_3}} : \vp$\`by Let (4,6)\\
\end{tabbing}
\end{proof}
\end{description}




\begin{theorem}
If $\G; \D_1,\D_2,\D_3 \vdash \ccase{e}{\{\overline{\rho_j\Rightarrow e_j}, \rho \Rightarrow
  E[e_1], \overline{\rho_k\Rightarrow e_k}\}}  : \vp$ and $e_1$ does not
use any pattern variables introduced by $\rho$, the case binder nor variables bound in
context $E[{-}]$
then 
$\G ; \D_1,\D_2,\D_3  \vdash \llet{x = e_1}{\ccase{e}{\{\overline{\rho_j\Rightarrow
           e_j}, \rho \Rightarrow E[x], \overline{\rho_k\Rightarrow e_k}\}}} : \vp$,
     for some fresh $x$.
              
   \end{theorem}
   
   \begin{proof}
   ~  
     \begin{tabbing}
       Subcase: $e$ is in WHNF\\
       (1) $\G;\D_1 \Vdash e:\s \gtrdot \ov{\D_i}$ \` by inversion\\
       (2) $\G ; \D_1 \vdash e : \s$ \` by inversion and constructor rule
       if needed\\
       (3) $\G,\var[z][\ov{\D_i}];\ov{\D_i},\D_2,\D_3 \vdash_{alt} \rho_j
       \Rightarrow e' :^z_{\ov{\D_i}} \s \Mapsto \vp$ \` by inversion\\
       (4) $\ov{\judg[\G,z{:}_{\irr{\D_1}}\s][\irr{\D_1},\D_2,\D_3]{\rho\Rightarrow e'}{\s
           \Rrightarrow \vp}[alt][\irr{\D_1}][z]}$ \` by inversion\\
       (5) $e$ matches $\rho_j$ \` by inversion\\
       Subsubcase: $\rho_j$ corresponds to branch containing $E[e_1]$\\
       Subsubsubcase: (3) derived by $\textrm{AltN}_{\textrm{WHNF}}$\\
       $\judg[\G, z{:}_{\ov{\Delta_i}} \sigma,\ov{\xo},\ov{y_i{:}_{\D_i}\s_i}^n][\ov{\D_i},\D_2,\D_3]{E[e_1]}{\vp}$
       \` by inversion\\
       
       $\judg[\G, z{:}_{\ov{\Delta_i}} \sigma,\ov{\xo},\ov{y_i{:}_{\D_i}\s_i}^n][\D',\D_2]{e_1}{\sigma'}$
       \` by inversion, with $\D' \subseteq \ov{\D_i} \subseteq \D_1$\\
       $\judg[\G, x{:}_{\D',\D_2}\sigma', z{:}_{\ov{\Delta_i}} \sigma,\ov{\xo},\ov{y_i{:}_{\D_i},\s_i}^n][\D',\D_2]{x}{\sigma'}$
       \` by Var$_\Delta$, with $x$ fresh\\
      $\judg[\G][\D',\D_2]{e_1}{\sigma'}$
       \` by assumption\\
       $\judg[\G,
       x{:}_{\D',\D_2}\sigma', z{:}_{\ov{\Delta_i}} \sigma,\ov{\xo},\ov{y_i{:}_{\D_i}\s_i}^n][\ov{\D_i},\D_2,\D_3]{E[x]}{\vp}$
       \` by context instantiation\\
       $\G,x{:}_{\D',\D_2}\sigma',\var[z][\ov{\D_i}];\ov{\D_i},\D_2,\D_3 \vdash_{alt} \rho_j
       \Rightarrow E[x] :^z_{\ov{\D_i}} \s \Mapsto \vp$ \` by
       $\textrm{AltN}_{\textrm{WHNF}}$\\
       $\G,x{:}_{\D',\D_2}\sigma'; \D_1,\D_2,\D_3 \vdash \ccase{e}{\{\overline{\rho_j\Rightarrow e_j}, \rho \Rightarrow
  E[x], \overline{\rho_k\Rightarrow e_k}\}} : \vp$ \` by $\textrm{Case}_\textrm{WHNF}$\\
       $\G ; \D_1 , \D_2 , \D_3 \vdash \llet{\x[\D',\D_2] = e_1}{\ccase{e}{\{\overline{\rho_j\Rightarrow e_j}, \rho \Rightarrow
           E[x], \overline{\rho_k\Rightarrow e_k}\}}} : \vp$ \` by $\mathit{Let}$\\
       Subsubsubcase: (3) derived by $\textrm{Alt}0$\\
       $\judg[\subst{\G, z{:}_{\ov{\Delta_i}} \sigma}{\cdot}{\ov{\D_i}}_z,\ov{\xo}][\subst{\ov{\D_i},\D_2,\D_3}{\cdot}{\ov{\D_i}}]{E[e_1]}{\vp}$
       \` by inversion\\
       $\judg[\G,z{:}_{\cdot}\s,\ov{\xo}][\D_2]{e_1}{\sigma'}$
       \` by inversion\\
       $\judg[\G][\D_2]{e_1}{\sigma'}$ \` by assumption\\
       $\judg[\G,x{:}_{\D_2}\sigma' , z{:}_{\cdot}\s,\ov{\xo}][\D_2]{x}{\sigma'}$ \` by Var$_\Delta$, with $x$ fresh\\
       $\judg[\subst{\G,x{:}_{\D_2}\sigma', z{:}_{\ov{\Delta_i}}
         \sigma }{\cdot}{\ov{\D_i}}_z,\ov{\xo}][\subst{\ov{\D_i},\D_2,\D_3}{\cdot}{\ov{\D_i}}]{E[x]}{\vp}$
       \` by context instantiation\\
             $\G,x{:}_{\D_2}\sigma'; \D_1,\D_2,\D_3 \vdash \ccase{e}{\{\overline{\rho_j\Rightarrow e_j}, \rho \Rightarrow
  E[x], \overline{\rho_k\Rightarrow e_k}\}} : \vp$ \` by $\textrm{Alt}0$ and
$\textrm{Case}_\textrm{WHNF}$\\
$\G ; \D_1 , \D_2 , \D_3 \vdash \llet{\x[\D_2] = e_1}{\ccase{e}{\{\overline{\rho_j\Rightarrow e_j}, \rho \Rightarrow
           E[x], \overline{\rho_k\Rightarrow e_k}\}}} : \vp$ \` by
       $\mathit{Let}$\\
       Subsubsubcase: (3) derived by $\textrm{Alt}\_$\\
       $\G , z{:}_{\ov{\Delta_i}} \sigma; \D_2,\D_3 \vdash E[e_1] : \vp$ \` by inversion\\
       $\judg[\G , z{:}_{\ov{\Delta_i}} \sigma][\D_2]{e_1}{\sigma'}$
       \` by inversion\\
       $\judg[\G, , z{:}_{\ov{\Delta_i}} \sigma ,x{:}_{\D_2}\sigma'][\D_2]{x}{\sigma'}$ \` by Var$_\Delta$, with $x$ fresh\\
       $\G, z{:}_{\ov{\Delta_i}} \sigma ,x{:}_{\D_2}\sigma'; \D_2,\D_3 \vdash E[e_1] : \vp$ \` by
       context instantiation\\
       $\G,x{:}_{\D_2}\sigma'; \D_1,\D_2,\D_3 \vdash \ccase{e}{\{\overline{\rho_j\Rightarrow e_j}, \rho \Rightarrow
  E[x], \overline{\rho_k\Rightarrow e_k}\}} : \vp$ \` by $\textrm{Alt}\_$ and
$\textrm{Case}_\textrm{WHNF}$\\
       $\G ; \D_1 , \D_2 , \D_3 \vdash \llet{\x[\D_2] = e_1}{\ccase{e}{\{\overline{\rho_j\Rightarrow e_j}, \rho \Rightarrow
           E[x], \overline{\rho_k\Rightarrow e_k}\}}} : \vp$ \` by
       $\mathit{Let}$\\
       Subsubcase: $\rho_j$ does not correspond to branch containing
       $E[e_1]$\\
       (6) $\judg[\G,z{:}_{\irr{\D_1}}\s][\irr{\D_1},\D_2,\D_3]{\rho\Rightarrow E[e_1]}{\s
         \Rrightarrow \vp}[alt][\irr{\D_1}][z]$ \` this subsubcase\\
       Subsubsubcase: (6) derived by $\textrm{AltN}_{\textrm{Not
           WHNF}}$\\
       $\judg[\G, z{:}_{\irr{\D_1}}\s,\ov{\xo},\ov{y_i{:}_{\D_i}\s_i}][\irr{\D_1},\D_2,\D_3]{E[e_1]}{\vp}$
       and $\ov{\D_i} = \ov{\lctag{\D_1}{K_i}}^n$ \` by inversion\\
       $\judg[\G,
       z{:}_{\irr{\D_1}}\s,\ov{\xo},\ov{y_i{:}_{\D_i}\s_i}][\D_2]{e_1}{\sigma'}$
       \` by inversion\\
       $\judg[\G,x{:}_{\D_2}\sigma',
       z{:}_{\irr{\D_1}}\s,\ov{\xo},\ov{y_i{:}_{\D_i}\s_i}][\D_2]{x}{\sigma'}$
       \` by Var$_\Delta$, with $x$ fresh\\
       $\judg[\G, x{:}_{\D_2}\sigma', z{:}_{\irr{\D_1}}\s,\ov{\xo},\ov{y_i{:}_{\D_i}\s_i}][\irr{\D_1},\D_2,\D_3]{E[x]}{\vp}$
       and $\ov{\D_i} = \ov{\lctag{\D_1}{K_i}}^n$ \` by context
       instantiation\\
         $\G,x{:}_{\D_2}\sigma'; \D_1,\D_2,\D_3 \vdash \ccase{e}{\{\overline{\rho_j\Rightarrow e_j}, \rho \Rightarrow
  E[x], \overline{\rho_k\Rightarrow e_k}\}} : \vp$ \` by $\textrm{AltN}_{\textrm{Not
           WHNF}}$ and
       $\textrm{Case}_\textrm{WHNF}$\\
         $\G ; \D_1 , \D_2 , \D_3 \vdash \llet{\x[\D_2] = e_1}{\ccase{e}{\{\overline{\rho_j\Rightarrow e_j}, \rho \Rightarrow
           E[x], \overline{\rho_k\Rightarrow e_k}\}}} : \vp$ \` by
       $\mathit{Let}$\\
       Subsubsubcase: (6) derived by $\textrm{Alt}\_$ or
       $\textrm{Alt}0$\\
       Identical to subsubsubcases above.\\
       Subcase: $e$ is not in WHNF\\
       (1) $\G ; \D_1 \vdash e : \s$ \` by inversion\\
       (2) $\ov{\judg[\G,z{:}_{\irr{\D_1}}\s][\irr{\D_1},\D_2,\D_3]{\rho\Rightarrow
           e'}{\s \Rrightarrow \vp}[alt][\irr{\D_1}][z]}$ \` by
       inversion\\
       (3) $\judg[\G,z{:}_{\irr{\D_1}}\s][\irr{\D_1},\D_2,\D_3]{\rho\Rightarrow
           E[e_1]}{\s \Rrightarrow \vp}[alt][\irr{\D_1}][z]$ \` by
         inversion\\
       Subsubcase: (3) derived by $\textrm{AltN}_{\textrm{Not
           WHNF}}$, $\textrm{Alt}\_$ or
       $\textrm{Alt}0$\\
       Identical to Subsubsubcases above.
     \end{tabbing}

   \end{proof}
%%% Local Variables:
%%% mode: latex
%%% TeX-master: "../../../icfp"
%%% End:
