
% ROMES: This one is pretty much complete, there are no pending todos. If you
% spot a mistake let me know.

\begin{lemma}[Substitution of unrestricted variables preserves typing]
\emph{If $\Gamma, x{:}_\omega\sigma \vdash e : \varphi$ and $\Gamma' \vdash e' : \sigma$ and $\hasnolinearvars{\Gamma'}$ then $\Gamma,\Gamma' \vdash e[e'/x] : \varphi$.}
\end{lemma}

\begin{proof}
By structural induction on the first derivation.

\begin{description}

\item[Case:] $Var_\omega$
\begin{tabbing}
  (1) $\Gamma, x{:}_\omega\sigma \vdash x : \sigma$\\
  (2) $\G' \vdash e' : \s$\\
  (3) $\hasnolinearvars{\Gamma}$ \` by inversion on ($Var_\omega$)\\
  (4) $x[e'/x] = e'$ \` by def. of substitution\\
  (5) $\G' \vdash e' : \sigma$ \` by (2)\\
  (6) $\G, \G' \vdash e' : \sigma$ \` by $Weaken_\omega$ (3)\\
\end{tabbing}

\item[Case:] $Var_\omega$
\begin{tabbing}
  (1) $\G, \xo \vdash y : \vp$\\
  (2) $\G' \vdash e' : \s$\\
  (3) $\hasnolinearvars{\G'}$\\
  (3) $y[e'/x] = y$ \` by def. of substitution\\
  (4) $\G \vdash y : \vp$ \` by inversion on $Weaken_\omega$ (1)\\
  (5) $\G, \G' \vdash y : \vp$ \` by $Weaken_\omega$ (3)\\
\end{tabbing}

\item[Case:] $Var_1$
\begin{tabbing}
  (1) Impossible. The context in $Var_1$ is empty.
\end{tabbing}

\item[Case:] $Var_\Delta$
\begin{tabbing}
  (1) Impossible. The context in $Var_\Delta$ only contains linear variables.
\end{tabbing}

\item[Case:] $Weaken_\omega$
\begin{tabbing}
  (1) $\G, \xo, \y[\omega][\s'] \vdash e : \vp$\\
  (2) $\G' \vdash e' : \s$ \`\\
  (3) $\hasnolinearvars{\G'}$ \`\\
  (4) $\G, \xo \vdash e : \vp$ \` by inversion on $Weaken_\omega$\\
  (5) $\G, \G' \vdash e[e'/x] : \vp$ \` by induction hypothesis (2,3,4)\\
  (6) $\G, \y[\omega][\s'], \G' \vdash e[e'/x] : \vp$ by $Weaken_\omega$\\
\end{tabbing}

\item[Case:] $Weaken_\Delta$
\begin{tabbing}
  (1) $\G, \xo, \y[\Delta][\s'] \vdash e : \vp$ \` by assumption\\
  (2) $\G' \vdash e' : \s$ \` by assumption\\
  (3) $\hasnolinearvars{\G'}$ \` by assumption\\
  (4) $\G, \xo \vdash e : \vp$ \` by inversion on $Weaken_\Delta$\\
  (5) $\G, \G' \vdash e[e'/x] : \vp$ \` by induction hypothesis (2,3,4)\\
  (6) $\G, \y[\Delta][\s'], \G' \vdash e[e'/x] : \vp$ by $Weaken_\Delta$\\
\end{tabbing}

\item[Case:] $Contract_\omega$
\begin{tabbing}
  (1) $\G, \xo, \y[\omega][\s'] \vdash e : \vp$\\
  (2) $\G' \vdash e' : \s$ \`\\
  (3) $\hasnolinearvars{\G'}$\\
  (4) $\G, \xo, \y[\omega][\s'], \y[\omega][\s'] \vdash e : \vp$ \` by inversion on $Contract_\omega$\\
  (5) $\G, \y[\omega][\s'], \y[\omega][\s'], \G' \vdash e[e'/x] : \vp$ \` by induction hypothesis (2,3,4)\\
  (6) $\G, \y[\omega][\s'], \G' \vdash e[e'/x] : \vp$ by $Contract_\omega$\\
\end{tabbing}

\item[Case:] $\Lambda I$
\begin{tabbing}
  (1) $\Gamma, \xo \vdash \Lambda p.~e : \forall p.~\varphi$\\
  (2) $\Gamma' \vdash e' : \sigma$ \\
  (3) $\hasnolinearvars{\G'}$\\
  (4) $\Gamma, \xo, p \vdash e : \varphi$ \` by inversion on $\Lambda I$\\
  (5) $p \notin \Gamma$ \` by inversion on $\Lambda I$\\
  (6) $\Gamma, p, \Gamma' \vdash e[e'/x] : \varphi$ \` by induction hypothesis by (2,3,4)\\
  (7) $\Gamma, \Gamma' \vdash \Lambda p.~e[e'/x] : \forall p.~\varphi$ \` by $\Lambda I$ (5,6)\\
  (8) $(\Lambda p.~e)[e'/x] = (\Lambda p.~e[e'/x])$ \` by def. of substitution\\
\end{tabbing}

\item[Case:] $\Lambda E$
\begin{tabbing}
  (1) $\G, \xo \vdash e~\pi: \varphi[\pi/p]$\\
  (2) $\G' \vdash e' : \sigma$\\
  (3) $\hasnolinearvars{\G'}$\\
  (4) $\Gamma, \xo \vdash e : \forall p.~\varphi$ \` by inversion on $\Lambda E$\\
  (5) $\Gamma, \xo \vdash_{mult} \pi$ \` by inversion on $\Lambda E$\\
  (6) $\Gamma, \Gamma' \vdash e[e'/x] \forall p.~\varphi$ \` by induction hypothesis by (2,3,4)\\
  (7) $\Gamma, \Gamma' \vdash e[e'/x]~\pi : \varphi[\pi/p]$ \` by $\Lambda E$ (5,6)\\
  (8) $(e~\pi)[e'/x] = e[e'/x]~\pi$ \` by def. of substitution\\
\end{tabbing}

\item[Case:] $\lambda I$
\begin{tabbing}
  (1) $\G, \xo \vdash \lambda\y[\pi][\s'].~e : \s'\to_\pi\vp$\\
  (2) $\G' \vdash e' : \sigma$\\
  (3) $\hasnolinearvars{\G'}$\\
  (4) $\G, \xo, \y[\pi][\s'] \vdash e : \vp$ \` by inversion on $\lambda I$\\
  (5) $\G, \G', \y[\pi][\s'] \vdash e[e'/x] : \vp$ \` by induction hypothesis (2,3,4)\\
  (6) $\G, \G' \vdash \lambda\y[\pi][\s'].~e[e'/x] : \s' \to_\pi\vp$ \` by $\lambda I$\\
  (7) $(\lambda \y[\pi][\s'].~e)[e'/x] = (\lambda \y[\pi][\s'].~e[e'/x])$ \` by def. of subst.\\
\end{tabbing}

\item[Case:] $\lambda E_{1,p}$
\begin{tabbing}
  (1) $\G, \xo, \G'' \vdash e~e'' : \vp$\\
  (2) $\G' \vdash e' : \s$\\
  (3) $\hasnolinearvars{\G'}$\\
  (4) $\G, \xo, \xo, \G'' \vdash e~e'' : \vp$ \` by $Contract_\omega$\\
  (5) $\G, \xo \vdash e : \s'\to_{1,p}\vp$ \` by inversion on $\lambda E_{1,p}$\\
  (6) $\G'', \xo \vdash e'' : \s'$ \` by inversion on $\lambda E_{1,p}$\\
  (7) $\G, \G' \vdash e[e'/x] : \s'\to_{1,p}\vp$ \` by induction hypothesis (2,3,5)\\
  (8) $\G'', \G' \vdash e''[e'/x] : \s'$ \` by induction hypothesis (2,3,6)\\
  (9) $\G, \G'', \G', \G' \vdash e[e'/x]~e''[e'/x] : \vp$ \` by $\lambda E_{1,p}$ (7,8)\\
  (10) $\G, \G'', \G' \vdash e[e'/x]~e''[e'/x] : \vp$ \` by $Contract_\omega$ (3)\\
  (11) $(e~e'')[e'/x] = (e[e'/x]~e''[e'/x])$ \` by def. of subst.\\
\end{tabbing}

\item[Case:] $\lambda E_\omega$
\begin{tabbing}
    (1) $\G, \xo, \G'' \vdash e~e'' : \vp$\\
    (2) $\G' \vdash e' : \s$\\
    (3) $\hasnolinearvars{\G'}$\\
    (4) $\G, \xo, \xo, \G'' \vdash e~e'' : \vp$ \` by $Contract_\omega$\\
    (5) $\G, \xo \vdash e : \s'\to_\omega\vp$ \` by inversion on $\lambda E_\omega$\\
    (6) $\G'', \xo \vdash e'' : \s'$ \` by inversion on $\lambda E_\omega$\\
    (7) $\G'', \G'$~\textrm{has no linear vars} \` by inversion on $\lambda E_\omega$ and (3)\\
    (8) $\G, \G' \vdash e[e'/x] : \s'\to_1\vp$ \` by induction hypothesis (2,3,5)\\
    (9) $\G'', \G' \vdash e''[e'/x] : \s'$ \` by induction hypothesis (2,3,6)\\
    (10) $\G, \G'', \G', \G' \vdash e[e'/x]~e''[e'/x] : \vp$ \` by $\lambda E_\omega$ (7,8,9)\\
    (11) $\G, \G'', \G' \vdash e[e'/x]~e''[e'/x] : \vp$ \` by $Contract_\omega$ (3)\\
    (12) $(e~e'')[e'/x] = (e[e'/x]~e''[e'/x])$ \` by def. of subst.\\
\end{tabbing}

\item[Case:] $Let$
\begin{tabbing}
    (1) $\G, \G'', \D, \xo \vdash \llet{\yD = e}{e''} : \vp$\\
    (2) $\G' \vdash e' : \sigma$\\
    (3) $\hasnolinearvars{\G'}$\\
    (4) $\G, \G'', \D, \xo, \xo \vdash \llet{\yD = e}{e''} : \vp$ \` by $Contract_\omega$\\
    (5) $\G, \D, \xo ,\yD \vdash e'' \vp$ \` by inversion on $Let$\\
    (6) $\G'', \D, \xo \vdash e : \s'$ \` by inversion on $Let$\\
    (7) $\hasnolinearvars{\G''}$ \` by inversion on $Let$\\
    (8) $\G, \D, \yD, \G' \vdash e''[e'/x] : \vp$ \` by induction hypothesis (2,3,5)\\
    (9) $\G'', \D, \G' \vdash e[e'/x] : \s'$ \` by induction hypothesis (2,3,6)\\
    (10) $\hasnolinearvars{\G'', \G'}$ \` by (3,7)\\
    (11) $\G,\G'',\D,\G',\G' \vdash \llet{\yD = e[e'/x]}{e''[e'/x]}$ \` by $Let$ (8,9,10)\\
    (12) $\G,\G'',\D,\G' \vdash \llet{\yD = e[e'/x]}{e''[e'/x]}$ \` by $Contract_\omega$\\
    (13) $(\llet{\yD = e}{e''})[e'/x] = (\llet{\yD = e[e'/x]}{e''[e'/x]})$
\end{tabbing}

\item[Case:] $LetRec$
\begin{tabbing}
    (1) $\G, \ov{\G''}, \ov{\D}, \xo \vdash \lletrec{\ov{\yD = e}}{e''} : \vp$\\
    (2) $\G' \vdash e' : \sigma$\\
    (3) $\hasnolinearvars{\G'}$\\
    (4) $\G, \ov{\G''}, \ov{\D}, \xo, \ov{\xo} \vdash \lletrec{\ov{\yD = e}}{e''} : \vp$ \` by $Contract_\omega$\\
    (5) $\G, \ov{\D}, \ov{\yD}, \xo \vdash e'' : \vp$ \` by inversion on $LetRec$\\
    (6) $\ov{\hasnolinearvars{\G''}}$ \` by inversion on $LetRec$\\
    (7) $\ov{\G'', \D, \ov{\yD}, \xo \vdash e : \s'}$ \` by inversion on $LetRec$\\
    (8) $\G, \ov{\D}, \ov{\yD}, \G' \vdash e''[e'/x] : \vp$ \` by induction hypothesis (2,3,5)\\
    (9) $\ov{\G'', \D, \ov{\yD}, \G' \vdash e[e'/x] : \s'}$ \` by induction hypothesis (2,3,6)\\
    (10) $\ov{\hasnolinearvars{\G'',\G'}}$ \` by (2,6)\\
    (11) $\G, \ov{\G''}, \ov{\D}, \G', \ov{\G'} \vdash \lletrec{\ov{\yD = e[e'/x]}}{e''[e'/x]} : \vp$ \` by $LetRec$ (8,9,10)\\
    (12) $\G, \ov{\G''}, \ov{\D}, \G' \vdash \lletrec{\ov{\yD = e[e'/x]}}{e''[e'/x]} : \vp$ \` by $Contract_\omega$ (2)\\
    (13) $(\lletrec{\ov{\yD = e}}{e''})[e'/x] = (\lletrec{\ov{\yD = e[e'/x]}}{e''[e'/x]})$
\end{tabbing}

\item[Case:] $Case$
\begin{tabbing}
    (1) $\G, \G'', \xo \vdash \ccase{e}{\zDp \{\ov{\rho_i \to e''_i}\}} : \vp$\\
    (2) $\G' \vdash e' : \s$\\
    (3) $\hasnolinearvars{\G'}$\\
    (4) $\G, \G'', \xo, \ov{\xo} \vdash \ccase{e}{\zDp \{\ov{\rho_i \to
    e''_i}\}} : \vp$ \` by $Contract_\omega$ (2)\\
    (5) $\G, \xo \vdash e : \s'$ \` by inversion on $Case$\\
    (6) $\G, \G' \vdash e[e'/x] : \s'$ \` by induction hypothesis (2,3,5)\\
    (7) $\ov{\G'', \xo, \zDip \vdash_{alt} \rho_i \to e''_i :_{\D_i} \s' \Rightarrow \vp}$\` by inversion on $Case$\\
    (8) $\ov{\G'', \zDip, \G' \vdash_{alt} \rho_i \to e''_i[e'/x] :_{\D_i} \s' \Rightarrow \vp}$\` by unr. subst. sublemma (2,3,7)\\
    (9) $\G, \G'', \G', \G' \vdash \ccase{e[e'/x]}{\zDp \{\ov{\rho_i \to e''_i[e'/x]}\}} : \vp$\` by $Case$ (6,8)\\
    (10) $(\ccase{e[e'/x]}{\zDp \{\ov{\rho_i \to e''_i[e'/x]}\}}) = \ccase{e}{\zDp \{\ov{\rho_i \to e''_i}\}}[e'/x]$\\
\end{tabbing}
\end{description}

\end{proof}

\begin{sublemma}[Substitution of unrestricted variables on case alternatives
    preserves typing]
\emph{If $\G, \xo \vdash_{alt} \rho \to e :_\Delta \s \Rightarrow \vp$ and $\G' \vdash e' : \s$ and
    $\hasnolinearvars{\G'}$ then $\G, \G' \vdash_{alt} \rho \to e[e'/x] :_\Delta \s \Rightarrow \vp$}
\end{sublemma}

\begin{proof}
By structural induction on the $alt$ judgment.

\begin{description}
\item[Case:] $Alt$
\begin{tabbing}
    (1) $\G, \xo \vdash_{alt} K~\ov{y{:}_\pi\s''} \to e :_\Delta \s' \Rightarrow \vp$\\
    (2) $\G' \vdash e' : \s$\\
    (3) $\hasnolinearvars{\G'}$\\
    (4) $\G, \xo, \ov{\y[\pi][\s'']} \vdash e : \vp$ \` by inversion on $Alt$\\
    (5) $K : \ov{\s'' \to_\pi} \s' \in \G$\` by inversion on $Alt$\\
    (6) $\D = \ov{\y[\pi][\s'']}\!\upharpoonright_1$\` by inversion on $Alt$\\
    (7) $\G,\ov{\y[\pi][\s'']},\G' \vdash e[e'/x] : \vp$\` by unr. subst. lemma (2,3,4)\\
    (8) $\G, \G' \vdash_{alt} K~\ov{\y[\pi][\s'']} \to e[e'/x] :_\Delta \s' \Rightarrow \vp$\` by $Alt$ (5,6,7)\\
\end{tabbing}

\item[Case:] $Alt_\_$
\begin{tabbing}
    (1) $\G, \xo \vdash_{alt} \_ \to e :_{\Delta_s} \s' \Rightarrow \vp$\\
    (2) $\G' \vdash e' : \s$\\
    (3) $\hasnolinearvars{\G'}$\\
    (4) $\G, \D_s, \xo \vdash e : \vp$\` by inversion on $Alt_\_$\\
    (5) $\G, \G', \D_s \vdash e[e'/x] : \vp$ \` by unr. subst. lemma (2,3,4)\\
    (6) $\G ,\G' \vdash_{alt} \_ \to e[e'/x] :_{\Delta_s} \s' \Rightarrow \vp$\\
\end{tabbing}

\end{description}
\end{proof}
