
\DeltaSubstitutionLemma

\begin{proof}
By structural induction on the first derivation.

\begin{description}

\item[Case:] $\Lambda I$
\begin{tabbing}
    (1) $\G, \xD; \D, \D' \vdash \Lambda p.~e : \forall p.~\vp$\\
    (2) $\G; \D \vdash e' : \s$\\
    (3) $\G, p, \xD; \D, \D' \vdash e : \vp$ \` by inversion on $\Lambda I$\\
    (4) $\G, p; \D, \D' \vdash e[e'/x]$ \` by induction hypothesis (2,3)\\
    (5) $\G; \D, \D' \vdash \Lambda p.~e[e'/x] : \forall p.~\vp$ \` by $\Lambda I$ \\
    (6) $(\Lambda p.~e)[e'/x] = (\Lambda p.~e[e'/x])$ \` by def. of subst.\\
    (7) $\G; \D, \D' \vdash (\Lambda p.~e)[e'/x] : \forall p.~\vp$ \` by (5,6)\\
\end{tabbing}

\item[Case:] $\Lambda E$
\begin{tabbing}
    (1) $\G,\xD; \D,\D' \vdash e~\pi : \vp$\\
    (2) $\G; \D \vdash e' : \s$\\
    (3) $\G,\xD; \D, \D' \vdash e : \forall p.~\vp$ \` by inversion on $\Lambda E$\\
    (4) $\G \vdash_{mult} \pi$ \` by inversion on $\Lambda E$\\
    (5) $\G; \D, \D' \vdash e[e'/x] : \forall p.~\vp$ \` by induction hypothesis (2,3)\\
    (6) $\G; \D, \D' \vdash e[e'/x]~\pi : \vp$ by $\Lambda E$\\
    (7) $(e~\pi)[e'/x] = (e[e'/x]~\pi)$ \` by def. of subst.\\
    (6) $\G; \D, \D' \vdash (e~\pi)[e'/x] : \vp$ by (5,6)\\
\end{tabbing}

\item[Case:] $\lambda I_1$
\begin{tabbing}
    (1) $\G, \xD; \D, \D' \vdash \lambda \y[1][\s'].~e : \s' \to_1 \vp$\\
    (2) $\G; \D \vdash e' : \s$\\
    (3) $\G, \xD; \D, \y[1][\s'], \D' \vdash e : \vp$ \` by inversion on $\lambda I$\\
    (4) $\G; \D, \y[1][\s'], \D' \vdash e[e'/x] : \vp$ \` by induction hypothesis (2,3)\\
    (5) $\G; \D, \D' \vdash \lambda \y[1][\s'].~e[e'/x] : \s' \to_1 \vp$ \` by $\lambda I$\\
    (6) $(\lambda \y[1][\s'].~e[e'/x]) = (\lambda \y[1][\s'].~e)[e'/x]$ \` by def. of subst.\\
    (7) $\G; \D, \D' \vdash \lambda (\y[1][\s'].~e)[e'/x] : \s' \to_1 \vp$ \` by (4,5)\\
\end{tabbing}

\item[Case:] $\lambda I_\omega$
\begin{tabbing}
    (1) $\G, \xD; \D, \D' \vdash \lambda \y[\omega][\s'].~e : \s' \to_\omega \vp$\\
    (2) $\G; \D \vdash e' : \s$\\
    (3) $\G, \xD, \y[\omega][\s']; \D, \D' \vdash e : \vp$ \` by inversion on $\lambda I$\\
    (4) $\G, \y[\omega][\s']; \D, \D' \vdash e[e'/x] : \vp$ \` by induction hypothesis (2,3)\\
    (5) $\G; \D, \D' \vdash \lambda \y[\omega][\s'].~e[e'/x] : \s' \to_\omega \vp$ \` by $\lambda I$\\
    (6) $(\lambda \y[\omega][\s'].~e[e'/x]) = (\lambda \y[\omega][\s'].~e)[e'/x]$ \` by def. of subst.\\
    (7) $\G; \D, \D' \vdash \lambda (\y[\omega][\s'].~e)[e'/x] : \s' \to_\omega \vp$ \` by (4,5)\\
\end{tabbing}

% I don't think this is still relevant, because the context of the Δ subst. is now exactly the
% same and the thing being substituted, and in the Var omega case, the Δ context must be empty (meaning the substitute must also have Δ=empty).
% Previously, the subst. wouldn't work in the following case because the
% case-binder was handled differently. Now, the case-binder will only be empty
% if the pattern is empty, in which case all resources are deleted:
%
% The previous case would happen for example if K :: a %ω -> b %ω -> K a b in
% case K e1 e2 of z:{}
%   K x y -> e3
% The substitution of z could happen in a context with no linear variables, and eventually get to Var_\omega
% To handle this, we change the lemma to only account for non empty Delta
% environments, which will forbid this case
% Instead, we used to handle that subcase when we need it
%
% Cool. The separation we used to do between empty Delta vs non empty Delta
% in the type preservation is now explicit in the two alternative rules for
% constructor patterns (AltN vs Alt0).
\item[Case:] $Var_\omega$
\begin{tabbing}
    (1) $\G, \yo, \x[\cdot][\s]; \cdot \vdash y : \s'$\\
    (2) $\G; \cdot \vdash e' : \s$\\
    (3) $y[e'/x] = y$\\
    (4) $\G,\yo;\cdot \vdash y : \s'$\` by (1) and $Weaken_\D$\\
\end{tabbing}

\item[Case:] $Var_1$
\begin{tabbing}
  (1) $\G,\x[\y]; \y \vdash y : \s$\\
  (2) $\G; \y \vdash e' : \s$\\
  (3) $y[e'/x] = y$\\
  (4) $\G,\x[\y]; \y \vdash y : \s$\`by 1\\ 
  (5) $\G; \y\vdash y : \s$\` by $Weaken_\Delta$\\
\end{tabbing}

\item[Case:] $Var_\Delta$
\begin{tabbing}
    (1) $\G, \xD; \D \vdash y : \s$\\
    (2) $\G'; \D \vdash e' : \s$\\
    % what about Subcase $x != y$
    (3) $x[e'/x] = e'$\\
    (4) $\G'; \D \vdash e' : \s$\` by (2)\\
\end{tabbing}

\item[Case:] $Split$
\begin{tabbing}
    Trivial induction
\end{tabbing}

\item[Case:] $\lambda E_{1,p}$
\begin{tabbing}
    (1) $\G, \xD; \D,\D',\D'' \vdash e~e'' : \varphi$\\
    (2) $\G; \D \vdash e' : \sigma$\\
    Subcase $\D$ occurs in $e$\\
    (3) $\G, \xD; \D,\D' \vdash e : \s' \to_{1,p} \vp$\\
    (4) $\G, \xD; \D'' \vdash e'' : \s'$\\
    (5) $\G; \D'' \vdash e'' : \s'$\` by $Weaken_\D$\\
    (6) $\G; \D,\D' \vdash e[e'/x] : \s' \to_{1,p} \vp$ \` by i.h.\\
    (7) $\G;\D, \D', \D'' \vdash e[e'/x]~e'' : \vp$\` by ($\lambda E_{1,p}$)\\
    (8) $(e[e'/x]~e'')=(e~e'')[e'/x]$\` since $x$ cannot occur in $e''$\\
    Subcase $\D$ occurs in $e''$\\
    (3) $\G, \xD; \D' \vdash e : \s' \to_{1,p} \vp$\\
    (4) $\G; \D' \vdash e : \s' \to_{1,p} \vp$\` by $Weaken_\Delta$\\
    (5) $\G,\xD; \D, \D'' \vdash e'' : \s'$\\
    (6) $\G; \D, \D'' \vdash e''[e'/x] : \s'$\` by i.h.\\
    (7) $\G; \D,\D',\D'' \vdash (e~e''[e'/x]) : \vp$\` by ($\lambda E_{1,p}$)\\
    (8) $e~e''[e'/x] = (e~e'')[e'/x]$\`since $x$ does not occur in $e$\\
    Subcase $\D$ is split between $e$ and $e''$\\
    $x$ cannot occur in either, so the substitution is trivial, and $x$ can be weakened.

\end{tabbing}

\item[Case:] $\lambda E_\omega$
\begin{tabbing}
    (1) $\G, \xD; \D, \D' \vdash e~e'' : \vp$\\
    (2) $\G; \D \vdash e' : \s$\\
    (3) $\D$ cannot occur in $e''$\\
    (4) $\G, \xD; \D, \D' \vdash e : \s' \to_\omega \vp$\` by inv. on $\lambda E_\omega$\\
    (5) $\G; \cdot \vdash e'' : \s'$ \` by inv. on $\lambda E_\omega$\\
    (6) $\G; \D, \D' \vdash e[e'/x] : \s' \to_\omega \vp$ \` by induction hypothesis (2,4)\\
    (7) $\G; \D, \D' \vdash e[e'/x]~e'' : \vp$\` by $\lambda E_\omega$ (5,6)\\
    (8) $e[e'/x]~e'' = (e~e'')[e'/x]$\` $x$ does not occur in $e''$ by (3)\\
\end{tabbing}

% In Let, LetRec and Case, we still use the old lemma where the $e'$ is typed
% with $\Delta$. I think to make this correct wrt to the new lemma, we'd need
% $\Delta''$ instead (we can't get rid of it, bc the linear vars in the subst. are important).
% But the proof's general idea is here. It might even be good enough.
\item[Case:] $Let$
\begin{tabbing}
    (1) $\G; \D \vdash e' : \s$\\
    Subcase $\D$ occurs in $e$\\
    (2) $\G, \xD; \D, \D', \D'' \vdash \llet{\y[\D,\D'][\s'] = e}{e''} : \vp$\\
    (3) $\G, \xD; \D, \D' \vdash e : \s'$\` by inversion on (let)\\
    (4) $\G, \xD,\y[\D,\D'][\s']; \D,\D', \D'' \vdash e'' : \vp$\` by inversion on (let)\\
    (5) $\G,\y[\D,\D'][\s']; \D,\D', \D'' \vdash e'' : \vp$\` by $Weaken_\Delta$ (admissible)\\
    (6) $\G; \D,\D' \vdash e[e'/x] : \s'$\` by induction hypothesis (1,3)\\
    (7) $\G; \D,\D',\D'' \vdash \llet{\y[\D,\D'][\s'] = e[e'/x]}{e''} : \vp$\` by (let) (5,6)\\
    (8) $\llet{\y[\D,\D'][\s'] = e[e'/x]}{e''} = (\llet{\y[\D,\D'][\s'] = e}{e''})[e'/x]$\\\` since $x$ cannot occur in $e''$\\
    Subcase $\D$ occurs in $e''$\\
    (2) $\G, \xD; \D, \D', \D'' \vdash \llet{\y[\D'][\s'] = e}{e''} : \vp$\\
    (3) $\G, \xD; \D' \vdash e : \s'$\` by inversion on (let)\\
    (4) $\G; \D' \vdash e : \s'$\` by $Weaken_\Delta$\\
    (5) $\G,\xD,\y[\D'][\s']; \D,\D',\D'' \vdash e'' : \vp$\` by inversion on (let)\\
    (6) $\G,\y[\D'][\s']; \D,\D',\D'' \vdash e''[e'/x] : \vp$\` by i.h. (1,5)\\
    (7) $\G;\D,\D',\D'' \vdash \llet{\y[\D'][\s'] = e}{e''[e'/x]} : \vp$\` by (let)\\
    (8) $\llet{\y[\D'][\s'] = e}{e''[e'/x]} = (\llet{\y[\D'][\s'] = e}{e''})[e'/x]$\\\` since $x$ cannot occur in $e$\\
    Subcase $\D$ is split between $e$ and $e''$\\
    $x$ cannot occur in either, so the substitution is trivial, and $x$ can be weakened.
\end{tabbing}

\item[Case:] LetRec
\begin{tabbing}
    (1) $\G; \D \vdash e' : \s$\\
    Subcase $\D$ occurs in $\ov{e_i}$\\
    (2) $\G,\xD; \D, \D', \D'' \vdash \lletrec{\ov{\var[y_i][\D,\D'][\s_i'] = e_i}}{e''} : \vp$\\
    (3) $\G,\xD,\ov{\var[y_i][\D,\D'][\s'_i]}; \D,\D',\D'' \vdash e'' : \vp$\` by inversion on (let)\\
    (4) $\G,\ov{\var[y_i][\D,\D'][\s'_i]}; \D,\D',\D'' \vdash e'' : \vp$\` by $Weaken_\Delta$\\
    (5) $\ov{\G,\xD,\ov{\var[y_i][\D,\D'][\s'_i]}; \D, \D' \vdash e_i : \s'_i}$\` by inversion on (let)\\
    (6) $\ov{\G,\ov{\var[y_i][\D,\D'][\s'_i]}; \D,\D' \vdash e_i[e'/x] : \s'_i}$\` by induction hypothesis (1,5)\\
    (7) $e''[e'/x] = e''$\` since $x$ cannot occur in $e''$\\
    (8) $\G; \D,\D',\D'' \vdash \lletrec{\ov{\var[y_i][\D,\D'][\s_i'] = e_i[e'/x]}}{e''} : \vp$\` by (let) (4,6)\\
    Subcase $\D$ occurs in $e''$\\
    (2) $\G, \xD; \D, \D', \D'' \vdash \lletrec{\ov{\var[y_i][\D'][\s_i'] = e_i}}{e''} : \vp$\\
    (3) $\ov{\G,\xD,\ov{\var[y_i][\D'][\s'_i]}; \D' \vdash e_i : \s'_i}$\` by inversion on (let)\\
    (4) $\ov{\G,\ov{\var[y_i][\D'][\s'_i]}; \D' \vdash e_i : \s'_i}$\` by $Weaken_\Delta$\\
    (6) $\G,\xD,\ov{\var[y_i][\D'][\s'_i]}; \D,\D',\D'' \vdash e'' : \vp$\` by inversion on (let)\\
    (7) $\G,\ov{\var[y_i][\D'][\s'_i]}; \D,\D',\D'' \vdash e''[e'/x] : \vp$\` by i.h. (1,6)\\
    (8) $\ov{e_i[e'/x] = e_i}$\` since $x$ cannot occur in $\ov{e_i}$\\
    (9) $\G;\D,\D',\D'' \vdash \lletrec{\ov{\var[y_i][\D'][\s'_i] = e_i}}{e''[e'/x]} : \vp$\` by (let)\\
    Subcase $\D$ is split between $e$ and $e''$\\
    $x$ cannot occur in either, so the substitution is trivial, and $x$ can be weakened.
\end{tabbing}

\item[Case:] CaseWHNF
\begin{tabbing}
    (1) $\G; \D \vdash e' : \s$\\
    Subcase $\D$ occurs in $e$\\
    (2) $\G,\xD;\D,\D',\D'' \vdash \ccase{e}{\z[\D,\D'][\s']~\{\ov{\rho \to e''}\}} : \vp$\\
    (3) $e$ is in WHNF\\
    (4) $\G,\xD;\D,\D' \vdash e : \s'$\\
    (5) $\ov{\G,\xD,\z[\D,\D'][\s']; \D,\D',\D'' \vdash_{alt} \rho \to e'' :^z_{\D,\D'} : \s' \Rightarrow \vp}$\\
    (6) $\G;\D,\D' \vdash e[e'/x] : \s'$\` by i.h.\\
    (7) $\ov{\G,\z[\D,\D'][\s']; \D,\D',\D'' \vdash_{alt} \rho \to e''[e'/x] :^z_{\D,\D'} \s' \Rightarrow \vp}$\` by subst. of $\D$ vars on case alts\\
    (8) $\G;\D,\D',\D'' \vdash \ccase{e[e'/x]}{\z[\D,\D'][\s']~\{\ov{\rho \to e''[e'/x]}\}} : \vp$\` by $CaseWHNF$\\
    Subcase $\D$ does not occurs in $e$\\
    (2) $\G,\xD;\D,\D',\D'' \vdash \ccase{e}{\z[\D'][\s']~\{\ov{\rho \to e''}\}} : \vp$\\
    (3) $e$ is in WHNF\\
    (4) $\G,\xD;\D' \vdash e : \s'$\\
    (5) $\G;\D' \vdash e : \s'$\` by (admissible) $Weaken_\D$\\
    (6) $e[e'/x] = e$\` by $x$ cannot occur in $e$\\
    (7) $\ov{\G,\xD,\z[\D'][\s']; \D,\D',\D'' \vdash_{alt} \rho \to e'' :^z_{\D'} : \s' \Rightarrow \vp}$\\
    (8) $\ov{\G,\z[\D'][\s']; \D,\D',\D'' \vdash_{alt} \rho \to e''[e'/x] :^z_{\D'} \s' \Rightarrow \vp}$\` by subst. of $\D$ vars on case alts\\
    (9) $\G;\D,\D',\D'' \vdash \ccase{e[e'/x]}{\z[\D'][\s']~\{\ov{\rho \to e''[e'/x]}\}} : \vp$\` by $CaseWHNF$\\
    Subcase $\D$ is partially used in $e$\\
    This is like the subcase above, but consider $\D'$\\
    to contain some of part of $\D$ and $\D$ to refer to the other part only.
\end{tabbing}

\item[Case:] CaseNotWHNF
\begin{tabbing}
    (1) $\G;\D\vdash e' :\s$\\
    Subcase $\D$ occurs in $e$\\
    (2) $\G,\xD; \D, \D', \D'' \vdash \ccase{e}{\z[\irr{\D,\D'}][\s']~\{\ov{\rho\to e''}\}}$\\
    (3) $\G,\xD; \D, \D' \vdash e : \s'$\` by inv.\\
    (4) $\G; \D,\D' \vdash e[e'/x] : \s'$\` by i.h.\\
    (5) $\ov{\G,\xD,\z[\irr{\D,\D'}][\s']; [\D,\D'],\D'' \vdash_{alt} \rho \to e'' :^z_{\irr{\D,\D'}} \s'\Rightarrow\vp}$\` by inv.\\
    (6) $e''[e'/x] = e$\` by $x$ cannot occur in $\ov{e''}$ since $\D$ is not available (only $\irr{\D}$)\\
    (7) $\ov{\G,\z[\irr{\D,\D'}][\s']; [\D,\D'],\D'' \vdash_{alt} \rho \to e'' :^z_{\irr{\D,\D'}} \s'\Rightarrow\vp}$\` by (admissible) $Weaken_\Delta$\\
    (8) $\G; \D, \D', \D'' \vdash \ccase{e[e'/x]}{\z[\irr{\D,\D'}][\s']~\{\ov{\rho\to e''}\}}$\`by $CaseNotWHNF$\\
    Subcase $\D$ does not occur in $e$\\
    (2) $\G,\xD; \D, \D', \D'' \vdash \ccase{e}{\z[\irr{\D'}][\s']~\{\ov{\rho\to e''}\}}$\\
    (3) $\G,\xD; \D' \vdash e : \s'$\` by inv.\\
    (4) $\G; \D' \vdash e : \s'$\` by weaken\\
    (5) $e[e'/x] = e$\` by x cannot occur in $e$\\
    (5) $\ov{\G,\xD,\z[\irr{\D'}][\s']; \D,[\D'],\D'' \vdash_{alt} \rho \to e'' :^z_{\irr{\D'}} \s'\Rightarrow\vp}$\` by inv.\\
    (7) $\ov{\G,\z[\irr{\D'}][\s']; \D,[\D'],\D'' \vdash_{alt} \rho \to e''[e'/x] :^z_{\irr{\D'}} \s'\Rightarrow\vp}$\\\` by subst. of $\D$-vars in case alternatives\\
    (8) $\G; \D, \D', \D'' \vdash \ccase{e}{\z[\irr{\D,\D'}][\s']~\{\ov{\rho\to e''[e'/x]}\}}$\`by $CaseNotWHNF$\\
    Subcase $\D$ is partially used in $e$\\
    This is like the subcase above, but consider $\D'$\\
    to contain some of part of $\D$ and $\D$ to refer to the other part only.
\end{tabbing}

\end{description}

\end{proof}


\DeltaSubstitutionAltsLemma
\begin{proof}
By structural induction on the $alt$ judgment.

\begin{description}
\item[Case:] $AltN_{WHNF}$ (trivial induction)
\begin{tabbing}
  (1) $\G; \D \vdash e' : \s$\\
  (2) $\G,\xD; \D,\D' \vdash_{alt} \konstructor~\to e \prescript{\dag}{}{:^z_{\ov{\D_i}^n}} \s' \Rightarrow \vp$\\
  (3) $\G,\xD,\ov{\xo},\ov{y_i{:}_{\D_i}\s_i}; \D, \D' \vdash e : \vp$\` by inv.\\
  (4) $\G,\ov{\xo},\ov{y_i{:}_{\D_i}\s_i}; \D, \D' \vdash e[e'/x] : \vp$\` by i.h.\\
  (5) $\G; \D,\D' \vdash_{alt} \konstructor~\to e[e'/x] \prescript{\dag}{}{:^z_{\ov{\D_i}^n}} \s' \Rightarrow \vp$\` by $AltN$\\
\end{tabbing}

\item[Case:] $AltN_{Not WHNF}$ (trivial induction)
\begin{tabbing}
  (1) $\G; \D \vdash e' : \s$\\
  (2) $\G,\xD; \D,\D' \vdash_{alt} \konstructor~\to e \prescript{\ddag}{}{:^z_{\D_s}} \s' \Rightarrow \vp$\\
  (3) $\ov{\D_i} = \ov{\lctag{\D_s}{K_j}}$\`by inv.\\
  (4) $\G,\xD,\ov{\xo},\ov{y_i{:}_{\D_i}\s_i}; \D, \D' \vdash e : \vp$\` by inv.\\
  (5) $\G,\ov{\xo},\ov{y_i{:}_{\D_i}\s_i}; \D, \D' \vdash e[e'/x] : \vp$\` by i.h.\\
  (6) $\G; \D,\D' \vdash_{alt} \konstructor~\to e[e'/x] \prescript{\ddag}{}{:^z_{\D_s}} \s' \Rightarrow \vp$\` by $AltN$\\
\end{tabbing}

\item[Case:] $Alt0$
\begin{tabbing}
% Fault. Delta var subst. used to be unsound on this case.
% On one hand we (used to) need the $\G[\cdot/\D]$ subst to ensure the case
% binder became unrestricted inside of alternatives with no linear patterns, and
% on the other hand we CANNOT have this $\G[\cdot/\D]$ because it means some
% other variables also become unrestricted, and allow duplicate usage of
% resources. We need an alternative way to make the case-binder unrestricted
% while keeping the existing variables unusable inside of the case expression.
% Examples in the call-notes.
    (1) $\G; \D \vdash e' : \s$\\
    Subcase $\D$ occurs in scrutinee\\
    (2) $\G,\xD; \D,\D',\D'' \vdash_{alt} K~\ov{\x}~\to e :^z_{\D,\D'} \s' \Rightarrow \vp$\\
    (3) $(\G,\xD)[\cdot/\D,\D']_z; (\D,\D',\D'')[\cdot/\D,\D'] \vdash e : \vp$\\
    (4) $\G[\cdot/\D,\D']_z, \xD; \D'' \vdash e : \vp$\\\`by def. of $[]_z$ subst. and $[]$ subst.\\
    (5) $\G[\cdot/\D,\D']_z, \xD; \D'' \vdash e[e'/x] : \vp$\\\`by $x$ cannot occur in $e$ by $\D$ not available\\
    (6) $\G[\cdot/\D,\D']_z; \D'' \vdash e[e'/x] : \vp$\\\`by (admissible) $Weaken_\D$\\
    (7) $\cdot = (\D,\D')[\cdot/\D,\D']$\\
    (8) $\G[\cdot/\D,\D']_z; (\D,\D',\D'')[\cdot/\D,\D'] \vdash e[e'/x] : \vp$\\\`by (6,7)\\
    (9) $\G;\D,\D',\D'' \vdash_{alt} e[e'/x] :^z_{\D,\D'} \s' \Rightarrow \vp$\\
    Subcase $\D$ does not occur in the scrutinee\\
    (2) $\G,\xD; \D,\D',\D'' \vdash_{alt} K~\ov{\x}~\to e :^z_{\D'} \s' \Rightarrow \vp$\\
    (3) $(\G,\xD)[\cdot/\D']_z; (\D,\D',\D'')[\cdot/\D'] \vdash e : \vp$\\
    (4) $\G[\cdot/\D']_z, \xD; \D,\D'' \vdash e : \vp$\\\`by def. of $[]_z$ subst. and $[]$ subst.\\
    (5) $\G[\cdot/\D']_z; \D,\D'' \vdash e[e'/x] : \vp$\` by $\D$-subst. lemma\\
    (6) $\cdot = \D'[\cdot/\D']$\\
    (7) $\G[\cdot/\D']_z; (\D,\D',\D'')[\cdot/\D'] \vdash e[e'/x] : \vp$\` by (5,6)\\
    (8) $\G;\D,\D',\D'' \vdash_{alt} \vdash e[e'/x] :^z_{\D'} \s' \Rightarrow \vp$\`by $Alt0$\\
    Subcase $\D$ is partially used in the scrutinee\\
    This is like the subcase above, but consider $\D'$\\
    to contain some of part of $\D$ and $\D$ to refer to the other part only.
\end{tabbing}

\item[Case:] $Alt_\_$ (trivial induction)
\begin{tabbing}
    (1) $\G;\D \vdash e' : \s$\\
    (2) $\G,\xD; \D,\D' \vdash_{alt} \_~\to e :^z_{\D_s} \s' \Rightarrow \vp$\\
    (3) $\G,\xD; \D,\D' \vdash e : \vp$\` by inv.\\
    (4) $\G; \D, \D' \vdash e[e'/x]] : \vp$\` by i.h.\\
    (5) $\G; \D,\D' \vdash_{alt} \_~\to e[e'/x] :^z_{\D_s} \s' \Rightarrow \vp$\` by $Alt_\_$\\
\end{tabbing}
\end{description}

\end{proof}

