\LinearSubstitutionLemma

% TODO: Short paragraph about the proof for case alternatives sublemma for
% Alt_0: It's hard because one must consider two different subcases, one in
% which $x$ is part of the scrutinee and other in which it isn't, to prove the goal...

% Template:
% (2) $\judg[][][]{}{}$\\

\begin{proof}
By structural induction on the first derivation.

\begin{description}

\item[Case:] $\Lambda I$
\begin{tabbing}
  (1) $\Gamma; \D, x{:}_1\sigma \vdash \Lambda p.~e : \forall p.~\varphi$\\
  (2) $\G; \D' \vdash e' : \sigma$\\
  (3) $\G, p; \D,x{:}_1\sigma \vdash e : \varphi$ \` by inversion on $\Lambda I$\\
  (4) $p \notin \Gamma$ \` by inversion on $\Lambda I$\\
  (5) $\G[\D'/x],p; \D,\D' \vdash e[e'/x] : \varphi$ \` by induction hypothesis by (2,3)\\
  (6) $\G[\D'/x];\D,\D' \vdash \Lambda p.~e[e'/x] : \forall p.~\varphi$ \` by $\Lambda I$ (4,5)\\
  (7) $(\Lambda p.~e)[e'/x] = (\Lambda p.~e[e'/x])$ \` by def. of substitution\\
\end{tabbing}

\item[Case:] $\Lambda E$
\begin{tabbing}
  (1) $\G; \D, x{:}_1\sigma \vdash e~\pi: \varphi[\pi/p]$\\
  (2) $\G; \D' \vdash e' : \sigma$\\
  (3) $\G; \D, \xl \vdash e : \forall p.~\varphi$ \` by inversion on $\Lambda E$\\
  (4) $\G \vdash_{mult} \pi$ \` by inversion on $\Lambda E$\\
  (5) $\G[\D'/x]; \D,\D' \vdash e[e'/x] : \forall p.~\varphi$ \` by induction hypothesis by (2,3)\\
  (6) $\G[\D'/x]; \D,\D' \vdash e[e'/x]~\pi : \varphi[\pi/p]$ \` by $\Lambda E$ (4,5)\\
  (7) $(e~\pi)[e'/x] = e[e'/x] \pi$ \` by def. of substitution\\
\end{tabbing}

\item[Case:] $\lambda I_1$
\begin{tabbing}
  (1) $\G; \D, \xl \vdash \lambda y{:}_1\sigma'.~e : \sigma' \to_1 \varphi$\\
  (2) $\G; \D' \vdash e' : \sigma$\\
  (3) $\G; \D, \xl, y{:}_1\sigma' \vdash e : \varphi$ \` by inversion on $\lambda I$\\
  (4) $\G[\D'/x]; \D, y{:}_1\sigma', \D' \vdash e[e'/x] : \varphi$ \` by induction hypothesis by (2,3)\\
  (5) $\G[\D'/x]; \D,\D' \vdash \lambda y{:}_1\sigma'.~e[e'/x] : \sigma' \to_1 \varphi$ \` by $\lambda I$ (4)\\
  (6) $(\lambda y{:}_1\sigma'.~e)[e'/x] = (\lambda y{:}_1\sigma'.~e[e'/x])$ \` by def. of substitution\\
\end{tabbing}

\item[Case:] $\lambda I_\omega$
\begin{tabbing}
  (1) $\G; \D, \xl \vdash \lambda y{:}_\omega\sigma'.~e : \sigma' \to_\omega \varphi$\\
  (2) $\G; \D' \vdash e' : \sigma$\\
  (3) $\G, y{:}_\omega\sigma'; \D, \xl \vdash e : \varphi$ \` by inversion on $\lambda I$\\
  (4) $\G[\D'/x], y{:}_\omega\sigma'; \D, \D' \vdash e[e'/x] : \varphi$ \` by induction hypothesis by (2,3)\\
  (5) $\G[\D'/x]; \D,\D' \vdash \lambda y{:}_\omega\sigma'.~e[e'/x] : \sigma' \to_1 \varphi$ \` by $\lambda I$ (4)\\
  (6) $(\lambda y{:}_\omega\sigma'.~e)[e'/x] = (\lambda y{:}_\omega\sigma'.~e[e'/x])$ \` by def. of substitution\\
\end{tabbing}

\item[Case:] $Var_1$
\begin{tabbing}
  (1) $\G;x{:}_1\sigma \vdash x : \sigma$\\
  (2) $\G;\D' \vdash e' : \sigma$\\
  (3) $\G[\D'/x]; \D' \vdash e' : \s$\` by weaken\\
  (4) $x[e'/x] = e'$ \` by def. of substitution\\
  % (4) $\cdot[\lin{\G'}/x] = \cdot$ \` by def. of substitution\\
  (5) $\G[\D'/x];\D' \vdash e' : \sigma$ \` by (3)\\
\end{tabbing}

\item[Case:] $Var_\omega$\\
  (1) Impossible. $x{:}_1\sigma$ can't be in the context.\\

\item[Case:] $Var_\Delta$
\begin{tabbing}
  (1) $\G,y{:}_{\Delta,\xl}\varphi; \D, x{:}_1\sigma \vdash y : \varphi$\\
  (2) $\G; \D' \vdash e' : \sigma$\\
  (3) $y[e'/x] = y$\\
  (4) $\G[\D'/x],y{:}_{\Delta,\D'}\varphi; \D,\D'; \vdash y : \varphi$ \` by $Var_\Delta$\\
\end{tabbing}

\item[Case:] $Split$
\begin{tabbing}
    Trivial induction
\end{tabbing}

\item[Case:] $\lambda E_1$
\begin{tabbing}
  (1) $\G; \D,\D'',\xl \vdash e~e'' : \vp$\\
  (2) $\G; \D' \vdash e' : \s$\\
  Subcase $x$ occurs in $e$\\
  (3) $\G; \D,\xl \vdash e : \s' \to_1 \vp$\` by inversion on $\lambda E_1$\\
  (4) $\G; \D'' \vdash e'' : \s'$\` by inversion on $\lambda E_1$\\
  (5) $\G[\D'/x]; \D, \D' \vdash e[e'/x] : \s' \to_1 \vp$\` by induction hypothesis (2,3)\\
  (6) $\G[\D'/x]; \D, \D', \D'' \vdash e[e'/x]~e'' : \vp$\` by $\lambda E_1$\\
  (7) $(e[e'/x]~e'') = (e~e'')[e'/x]$ \` because $x$ does not occur in $e''$\\
  Subcase $x$ occurs in $e''$\\
  (3) $\G; \D \vdash e : \s' \to_1 \vp$\` by inversion on $\lambda E_1$\\
  (4) $\G; \D'', \xl \vdash e'' : \s'$\` by inversion on $\lambda E_1$\\
  (5) $\G[\D'/x]; \D'',\D' \vdash e''[e'/x] : \s'$\` by induction hypothesis (2,4)\\
  (6) $\G[\D'/x]; \D,\D',\D'' \vdash e~e''[e'/x] : \vp$\` by $\lambda E_1$\\
  %(7) $\d[\D'/x] = \d$\` $x$ doesn't occur in $e$, so $\Delta$-bound vars in $e$ \\
  %    \` couldn't contain $x$ and still be well-typed.\\
  (7) $(e~e''[e'/x]) = (e~e'')[e'/x]$ \` because $x$ does not occur in $e$\\
\end{tabbing}

\item[Case:] $\lambda E_\omega$
\begin{tabbing}
  (1) $\G; \D, \xl \vdash e~e'' : \vp$\\
  (2) $\G; \D' \vdash e' : \s$\\
  (3) $x$ does not occur in $e''$\` by $e''$ linear context is empty\\
  (4) $\G; \D, \xl \vdash e : \s' \to_\omega \vp$\` by inversion on $\lambda E_\omega$\\
  (5) $\G; \cdot \vdash e'' : \s'$\` by inversion on $\lambda E_\omega$\\
  (6) $\G[\D'/x]; \D, \D' \vdash e[e'/x] : \s' \to_\omega \vp$\` by induction hypothesis (2,4)\\
  (7) $\G[\D'/x]; \D, \D' \vdash e[e'/x]~e'' : \vp$\` by $\lambda E_\omega$\\
  % (8) $\G''[\lin{\G'}/x] = \G''$\` $x$ doesn't occur in $e''$, so $\Delta$-bound vars in $e''$ \\
  %     \` couldn't contain $x$ and still be well-typed.\\
  (8) $(e[e'/x]~e'') = (e~e'')[e'/x]$ \` because $x$ does not occur in $e''$\\
\end{tabbing}

\item[Case:] $Let$
\begin{tabbing}
  (1) $\G; \D' \vdash e' : \s$\\
  Subcase $x$ occurs in $e$\\
  (2) $\G; \D, \xl, \D'' \vdash \llet{\y[\D,\xl][\s'] = e}{e''} : \vp$\\
  (3) $\G,\y[\D,\xl][\s']; \D, \xl, \D'' \vdash e'' : vp$\` by inversion on $Let$\\
  (4) $\G; \D, \xl \vdash e : \s'$\` by inversion on $Let$\\
  (5) $\G[\D'/x],\y[\D,\D'][\s']; \D, \D', \D'' \vdash e''[e'/x]$\` by induction hypothesis $(1,3)$\\
  (6) $\G[\D'/x]; \D, \D' \vdash e[e'/x] : \s'$ \` by induction hypothesis $(1,4)$\\
  % (8) $\hasnolinearvars{\G''[\lin{\G'}/x]}$\` by (2) and def. of env. subst.\\
  (7) $\G[\D'/x]; \D, \D', \D'' \vdash \llet{\y[\D,\D'][\s'] = e[e'/x]}{e''[e'/x]} : \vp$ \` (5,6) by $Let$\\
  % (10) $\G[\D'/x]; \D, \D' \vdash \llet{\y[\D,\D'][\s'] = e[e'/x]}{e''[e'/x]} : \vp$ \` by $Contract_\omega$\\
  % (11) $\Delta[\lin{\G'}/x] = \Delta$ \` $\Delta$ only has linear vars, by construction\\
  (8) $(\llet{\y[\D,\D'][\s'] = e[e'/x]}{e''[e'/x]}) = (\llet{\y[\D,\D'][\s'] = e}{e''})[e'/x]$ \` by subst.\\
  Subcase $x$ does not occur in $e$\\
  (2) $\G; \D, \D'', \xl  \vdash \llet{\yD = e}{e''} : \vp$\\
  (3) $\G,\yD; \D, \D'', \xl \vdash e'' : \vp$ \` by inversion on $Let$\\
  (4) $\G; \D \vdash e : \s'$ \` by inversion on $Let$\\
  (5) $\G[\D'/x],\yD; \D, \D', \D'' \vdash e''[e'/x] : \vp$\` by induction hypothesis (1,3)\\
  (6) $\G[\D'/x]; \D, \D', \D'' \vdash \llet{\yD = e}{e''[e'/x]} : \vp$ \` by $Let$ (2,5,6)\\
  % (7) $\D[\lin{\G'}/x] = \D$\` $\Delta$ only has linear vars, by construction\\
  % (8) $\G''[\lin{\G'}/x] = \G''$\` by (2) and $x \notin \Delta$ in this subcase,\\
  % \` $\G''$ can't have a $\Delta$-bound var mentioning $x$.\\
  (7) $\llet{\yD = e}{e''[e'/x]} = (\llet{\yD = e}{e''})[e'/x]$\` by $x$ does
  not occur in $e$\\
\end{tabbing}

\item[Case:] $LetRec$
\begin{tabbing}
  (1) $\G; \D' \vdash e' : \s$\\
  % (2) $\ov{\hasnolinearvars{\G''_i}}$\` by inversion on $LetRec$\\
  Subcase $\xl$ occurs in some $e_i$\\
  (2) $\G; \D, \xl, \D'' \vdash \lletrec{\ov{\var[y_i][\D,\xl][\s_i] = e_i}}{e''} : \vp$\\
  (3) $\G, \ov{\var[y_i][\D,\xl][\s_i]}; \D, \xl, \D'' \vdash e'' : \vp$\` by inversion on $LetRec$\\
  (4) $\ov{\G,\ov{\var[y_i][\D, \xl][\s_i]}; \D, \xl \vdash e_i : \s_i}$\` by inversion on $LetRec$\\
  (5) $\G[\D'/x], \ov{\var[y_i][\D, \D'][\s_i]}; \D, \D', \D'' \vdash e''[e'/x] : \vp$ \` by induction hypothesis (1,3)\\
  (6) $\ov{\G, \ov{\var[y_i][\D, \D'][\s_i]}; \D, \D' \vdash e_i[e'/x] : \s_i}$\` by induction hypothesis (1,4)\\
  (7) $\G[\D'/x]; \D, \D', \D'' \vdash \lletrec{\ov{\var[y_i][\D,\G'_1][\s_i] = e_i[e'/x]}}{e''[e'/x]} : \vp$\` by $LetRec$\\
  (8) $(\lletrec{\ov{\var[y_i][\D,\D'][\s_i] = e_i}}{e''})[e'/x] = \lletrec{\ov{\var[y_i][\D,\D'][\s_i] = e_i[e'/x]}}{e''[e'/x]}$\\
  Subcase $\xl$ does not occur in any $e_i$\\
  (2) $\G; \D, \xl, \D'' \vdash \lletrec{\ov{\var[y_i][\D][\s_i] = e_i}}{e''} : \vp$\\
  (3) $\G, \ov{\var[y_i][\D][\s_i]}; \D, \xl, \D'' \vdash e'' : \vp$\` by inversion on $LetRec$\\
  (4) $\ov{\G, \ov{\var[y_i][\D][\s_i]}; \D \vdash e_i : \s_i}$\` by inversion on $LetRec$\\
  (5) $\G[\D'/x], \ov{\var[y_i][\D][\s_i]}; \D, \D', \D'' \vdash e''[e'/x] : \vp$\` by i.h. (1,3)\\
  (6) $\G[\D'/x]; \D, \D', \D'' \vdash \lletrec{\ov{\var[y_i][\D][\s_i] = e_i}}{e''[e'/x]} : \vp$\` by $LetRec$\\
  (7) $\lletrec{\ov{\var[y_i][\D][\s_i] = e_i}}{e''[e'/x]} = (\lletrec{\ov{\var[y_i][\D][\s_i] = e_i}}{e''})[e'/x]$\` by subcase\\
\end{tabbing}

\item[Case:] $CaseWHNF$
\begin{tabbing}
  (1) $\judg[\G][\D']{e'}{\s}$\\
  Subcase $x$ occurs in $e$\\
  (2) $\judg[\G][\D,\xl,\D'']{\ccase{e}{\z[\D,\xl][\s']~\{\ov{\rho\to e''}\}}}{\vp}$\\
  (3) $e$ is in WHNF\\
  (4) $\judg[\G][\D,\xl]{e}{\s'}$\\
    (5) $\ov{\judg[\G,\zr{\D,\xl}{\s'}][\D,\xl,\D'']{\rho\to e''}{\s' \Longrightarrow \vp}[alt][\D,\xl][z]}$\\
  (6) $\judg[\subst{\G}{\D'}{x}][\D,\D']{e[e'/x]}{\vp}$\`by i.h.\\
    (7) $\ov{\judg[\subst{\G}{\D'}{x},\zr{\D,\D'}{\s'}][\D,\D',\D'']{\rho\to e''[e'/x]}{\s' \Longrightarrow \vp}[alt][\D,\D'][z]}$\` by lin. subst. alts.\\
  (8) $\judg[\subst{\G}{\D'}{x}][\D,\D',\D'']{\ccase{e[e'/x]}{\z[\D,\D'][\s']~\{\ov{\rho\to e''[e'/x]}\}}}{\vp}$\\
  Subcase $x$ occurs in $\ov{e''}$\\
  (2) $\judg[\G][\D,\D'',\xl]{\ccase{e}{\z[\D][\s']~\{\ov{\rho\to e''}\}}}{\vp}$\\
  (3) $e$ is in WHNF\\
  (4) $\judg[\G][\D]{e}{\s'}$\\
    (5) $\ov{\judg[\G,\zr{\D}{\s'}][\D,\D'',\xl]{\rho\to e''}{\s' \Longrightarrow \vp}[alt][\D][z]}$\\
  (6) $e[e'/x] = e$\` by $x$ does not occur in $e$\\
    (7) $\ov{\judg[\subst{\G}{\D'}{x},\zr{\D}{\s'}][\D,\D'',\D']{\rho\to e''[e'/x]}{\s' \Longrightarrow \vp}[alt][\D][z]}$\`by i.h.\\
  (8) $\judg[\subst{\G}{\D'}{x}][\D,\D'',\D']{\ccase{e}{\z[\D][\s']~\{\ov{\rho\to e''[e'/x]}\}}}{\vp}$\\
\end{tabbing}

\item[Case:] $CaseNotWHNF$
    % TODO: I can also use congruence for the proof irrelevant stuff? (that is, instead of invoking the other lemma?)
\begin{tabbing}
  (1) $\judg[\G][\D']{e'}{\s}$\\
  Subcase $x$ occurs in $e$\\
    (2) $\judg[\G][\D,\xl,\D'']{\ccase{e}{\z[\irr{\D,\xl}][\s']~\{\ov{\rho\to e''}\}}}{\vp}$\\
    (3) $e$ is definitely not in WHNF\\
    (4) $\judg[\G][\D,\xl]{e}{\s'}$\`by inv.\\
    (5) $\ov{\judg[\G,\zr{\irr{\D,\xl}}{\s'}][\irr{\D,\xl},\D'']{\rho\to e''}{\s' \Longrightarrow \vp}[alt][\irr{\D,\xl}][z]}$\`by inv.\\
    (6) $\judg[\subst{\G}{\D'}{x}][\D,\D']{e[e'/x]}{\vp}$\`by i.h.\\
    (7) $\ov{\judg[\subst{\G}{\D'}{x},\zr{\irr{\D,\D'}}{\s'}][\irr{\D,\D'},\D'']{\rho\to e''[e'/x]}{\s' \Longrightarrow \vp}[alt][\irr{\D,\D'}][z]}$\\
    \` by subst. of p. irr. vars in alt.\\
    \` or, simply, congruence? \\
    \` (x only occurs in ctxts, so replace all xs by $\D'$, starting by $\G$)?\\
    (8) $\judg[\subst{\G}{\D'}{x}][\D,\D',\D'']{\ccase{e[e'/x]}{\z[\D,\D'][\s']~\{\ov{\rho\to e''[e'/x]}\}}}{\vp}$\\
  Subcase $x$ occurs in $\ov{e''}$\\
    (2) $\judg[\G][\D,\D'',\xl]{\ccase{e}{\z[\irr{\D}][\s']~\{\ov{\rho\to e''}\}}}{\vp}$\\
    (3) $e$ is definitely not in WHNF\\
    (4) $\judg[\G][\D]{e}{\s'}$\`by inv.\\
    (5) $\ov{\judg[\G,\zr{\irr{\D}}{\s'}][\irr{\D},\D'',\xl]{\rho\to e''}{\s' \Longrightarrow \vp}[alt][\irr{\D}][z]}$\`by inv.\\
    (6) $e[e'/x] = e$\` by $x$ does not occur in $e$\\
    (7) $\ov{\judg[\subst{\G}{\D'}{x},\zr{\irr{\D}}{\s'}][\irr{\D},\D'',\D']{\rho\to e''[e'/x]}{\s' \Longrightarrow \vp}[alt][\irr{\D}][z]}$\`by lin. subst. on alts\\
    (8) $\judg[\subst{\G}{\D'}{x}][\D,\D'',\D']{\ccase{e}{\z[\irr{\D}][\s']~\{\ov{\rho\to e''[e'/x]}\}}}{\vp}$\\
\end{tabbing}

% No longer a problem! It really is unsafe to have reverse-binder-swap in face of beta reduction
% \item[Case:] $CaseVar$
% \begin{tabbing}
%     Great! Substitution doesn't preserve types for this case...
% \end{tabbing}


\end{description}
\end{proof}

\begin{sublemma}[Substitution of linear variables on case alternatives
    preserves typing]
    If $\judg[\G][\D,\xl]{\rho\to e}{\s \Longrightarrow \vp}[alt][\D_s][z]$ and
    $\judg[\G][\D']{e'}{\s}$ and
    $\D_s \subseteq \D,x$ then
    $\judg[\subst{\G}{\D'}{x}][\D,\D']{\rho \to e[e'/x]}{\s \Longrightarrow \vp}[alt][\subst{\D_s}{\D'}{x}][z]$
\end{sublemma}

\begin{proof}
By structural induction on the $alt$ judgment.

\begin{description}
\item[Case:] $AltN_{WHNF}$
\begin{tabbing}
    (1) $\judg[\G][\D']{e'}{\s}$\\
    (2) $\judg[\G][\D,\xl]{\konstructor~\to e}{\s' \Longrightarrow \vp}[alt][\D_s][z][\dag]$\\
    (3) $\judg[\G,\ov{\xo},\ov{y_i{:}_{\D_i}\s_i}][\D,\xl]{e}{\vp}$\`by inv.\\
    (4) $\judg[\subst{\G}{\D'}{x},\ov{\xo},\ov{y_i{:}_{\subst{\D_i}{\D'}{x}}\s_i}][\D,\D']{e[e'/x]}{\vp}$\` by i.h.\\
    (5) $\judg[\subst{\G}{\D'}{x}][\D,\D']{\rho \to e[e'/x]}{\s' \Longrightarrow \vp}[alt][\subst{\D_s}{\D'}{x}][z][\dag]$\` by (4)\\
\end{tabbing}

\item[Case:] $AltN_{Not WHNF}$
\begin{tabbing}
    (1) $\judg[\G][\D']{e'}{\s}$\\
    (2) $\judg[\G][\D,\xl]{\konstructor~\to e}{\s' \Longrightarrow \vp}[alt][\D_s][z][\ddag]$\\
    % (3) $n > 0$\`by inv.\\
    (3) $\ov{\D_i}=\ov{\lctag{\D_s}{K_j}}^n$\`by inv.\\
    % (5) $\ov{\D_i\neq\cdot}$\\
    (4) $\judg[\G,\ov{\xo},\ov{y_i{:}_{\D_i}\s_i}][\D,\xl]{e}{\vp}$\`by inv.\\
    (5) $\judg[\subst{\G}{\D'}{x},\ov{\xo},\ov{y_i{:}_{\subst{\D_i}{\D'}{x}}\s_i}][\D,\D']{e[e'/x]}{\vp}$\` by i.h.\\
    (6) $\ov{\D_i[\D'/x]}=\ov{\lctag{\D_s[\D'/x]}{K_j}}^n$\`by (3) and cong.\\
    (7) $\judg[\subst{\G}{\D'}{x}][\D,\D']{\rho \to e[e'/x]}{\s' \Longrightarrow \vp}[alt][\subst{\D_s}{\D'}{x}][z][\ddag]$\` by (5,6)\\
\end{tabbing}

\item[Case:] $Alt0$
    This is one of the most interesting proof cases, and particularly hard to prove.
        \begin{itemize}
            \item The first insight is to divide the proof into two subcases, accounting
                for when the scrutinee (and hence $\D_s$) contains the linear resource and when it does not.
            \item The second insight is to recall that $\D$ and $\D'$ are
                disjoint to be able to prove the subcase in which $x$ does not
                occur in the scrutinee
            \item The third insight is to \emph{create} linear resources
                seemingly out of nowhere \emph{under a substitution that
                removes them}. We see this happen in the case where $x$ occurs
                in the scrutinee, for both the linear and affine contexts (see (5,6)).
                We must also see that we can swap $x$ for $\D'$ if neither can occur (see (7)).
        \end{itemize}
\begin{tabbing}
  (1) $\judg[\G][\D']{e'}{\s}$\\
  Subcase $x$ occurs in scrutinee\\
    (2) $\judg[\G][\D,\xl]{K~\ov{\xo}~\to e}{\s' \Longrightarrow \vp}[alt][\D_s,\xl][z]$\\
    (2.5) $\judg[\subst{\G}{\cdot}{\D_s,x}_z,\ov{\xo}][\subst{(\D,\xl)}{\cdot}{\D_s,x}]{e}{\vp}$\`by inv.\\
    (3) $\judg[\subst{\G}{\cdot}{\D_s,x}_z,\ov{\xo}][\subst{\D}{\cdot}{\D_s}]{e}{\vp}$\\
    (4) $e[e'/x] = e$\` since $x$ cannot occur in $e$ (erased from cx)\\
    (5) $\D[\cdot/\D_s] = (\D,\D')[\cdot/\D_s,\D']$   \` by cong. of subst.\\
    (6) $\G[\cdot/\D_s,x]_z[\D'/x] = \G[\D'/x][\cdot/\D_s,\D']_z$\` by cong. of subst. and more\\
    (7) $\forall x,\D,\D',\G:x\notin\Delta \land \Delta'\not\subset\D \land \G;\D \vdash e :\s \Longrightarrow \G[\D'/x];\D \vdash e : \s$\` by Weaken\\
    \` and variables in $\G$ cannot occur in $e$ if they mention $x$ nor if they mention $\D'$ \\
    % (6) $\G[\cdot/\D_s,x]_z = \G[\D'/x][\cdot/\D_s,\D']_z$\` by cong. of subst.\\
    (8) $\judg[\subst{\subst{\G}{\D'}{x}}{\cdot}{\D_s,\D'}_z,\ov{\xo}][\subst{(\D,\D')}{\cdot}{\D_s,\D'}]{e[e'x]}{\vp}$\` by (4,5,6,7)\\\` and $x$ and $\D'$ are erased from ctx\\
    % (8) $\judg[\G,\ov{\xo}][\subst{(\D,\D')}{\cdot}{\D_s,\D'}][\subst{\subst{\G}{\D'}{x},\d'}{\cdot}{\D_s,\D'}]{e[e'x]}{\vp}$\` by $Weaken_\Delta$\\
    (9) $\judg[\subst{\G}{\D'}{x}][\D,\D']{K~\ov{\xo}~\to e[e'/x]}{\s' \Rightarrow \vp}[alt][\D_s,\D'][z]$\` by $Alt0$\\
  Subcase $x$ does not occur in scrutinee\\
    (2) $\judg[\G][\D,\xl]{K~\ov{\xo}~\to e}{\s' \Longrightarrow \vp}[alt][\D_s][z]$\\
    (3) $\judg[\subst{\G}{\cdot}{\D_s}_z,\ov{\xo}][\subst{\D}{\cdot}{\D_s},\xl]{e}{\vp}$\`by $x$ does not occur in $\D_s$ and inv.\\
    (4) $\judg[\subst{\subst{\G}{\D'}{x}}{\cdot}{\D_s}_z,\ov{\xo}][\subst{\D}{\cdot}{\D_s},\D']{e[e'/x]}{\vp}$\\\`by i.h. and $x$ does not occur in $\D_s$\\
    (5) $\judg[\subst{\subst{\G}{\D'}{x}}{\cdot}{\D_s}_z,\ov{\xo}][\subst{(\D,\D')}{\cdot}{\D_s}]{e[e'/x]}{\vp}$\\
    \`by $\D$ and $\D'$ being disjoint by hypothesis,\\
    \`and $\D_s$ being a subset of $\D$\\ % (CHECK: Done, we require this as requirement to invoke the lemma)\\
    (6) $\D_s[\D'/x] = \D_s$\`by $x$ does not occur in $\D_s$\\
    (7) $\judg[\subst{\G}{\D'}{x}][\D,\D']{K~\ov{\xo}~\to e[e'/x]}{\s' \Rightarrow \vp}[alt][\subst{\D_s}{\D'}{x}][z]$\\
\end{tabbing}

\item[Case:] $Alt\_$ (trivial induction)
\begin{tabbing}
    (1) $\judg[\G][\D']{e'}{\s}$\\
    (2) $\judg[\G][\D,\xl]{\_~\to e}{\s' \Longrightarrow \vp}[alt][\D_s][z]$\\
    (3) $\judg[\G][\D,\xl]{e}{\vp}$\\
    (4) $\judg[\subst{\G}{\D'}{x}][\D,\D']{e[e'/x]}{\vp}$\\
    (5) $\judg[\subst{\G}{\D'}{x}][\D,\D']{\_~\to e[e'/x]}{\s' \Rightarrow \vp}[alt][\D_s,\D'][z]$\\
\end{tabbing}

\end{description}

\end{proof}

