
% ROMES: This one is pretty much complete, there are no pending todos. If you
% spot a mistake let me know.

\begin{lemma}[Substitution of unrestricted variables preserves typing]
\emph{If $\Gamma, x{:}_\omega; \Delta \sigma \vdash e : \varphi$ and $\Gamma; \cdot \vdash e' : \sigma$ then $\G,\D \vdash e[e'/x] : \varphi$.}
\end{lemma}

\begin{proof}
By structural induction on the first derivation.

\begin{description}

\item[Case:] $\Lambda I$
\begin{tabbing}
  (1) $\G, \xo; \D \vdash \Lambda p.~e : \forall p.~\varphi$\\
  (2) $\G; \cdot \vdash e' : \sigma$ \\
  (3) $\G, \xo, p; \D \vdash e : \varphi$ \` by inversion on $\Lambda I$\\
  (4) $p \notin \G$ \` by inversion on $\Lambda I$\\
  (5) $\G, p; \D \vdash e[e'/x] : \varphi$ \` by induction hypothesis by (2,3)\\
  (6) $\G; \D \vdash \Lambda p.~e[e'/x] : \forall p.~\varphi$ \` by $\Lambda I$ (4,5)\\
  (7) $(\Lambda p.~e)[e'/x] = (\Lambda p.~e[e'/x])$ \` by def. of substitution\\
\end{tabbing}

\item[Case:] $\Lambda E$
\begin{tabbing}
  (1) $\G, \xo; \D \vdash e~\pi: \varphi[\pi/p]$\\
  (2) $\G; \cdot \vdash e' : \sigma$\\
  (3) $\G, \xo; \D \vdash e : \forall p.~\varphi$ \` by inversion on $\Lambda E$\\
  (4) $\G \vdash_{mult} \pi$ \` by inversion on $\Lambda E$\\
  (5) $\G; \D \vdash e[e'/x] \forall p.~\varphi$ \` by induction hypothesis by (2,3)\\
  (6) $\G; \D \vdash e[e'/x]~\pi : \varphi[\pi/p]$ \` by $\Lambda E$ (4,5)\\
  (7) $(e~\pi)[e'/x] = e[e'/x]~\pi$ \` by def. of substitution\\
\end{tabbing}

\item[Case:] $\lambda I_1$
\begin{tabbing}
  (1) $\G, \xo; \D \vdash \lambda\y[1][\s'].~e : \s'\to_1\vp$\\
  (2) $\G; \cdot \vdash e' : \sigma$\\
  (3) $\G, \xo; \D, \y[1][\s'] \vdash e : \vp$ \` by inversion on $\lambda I_1$\\
  (4) $\G; \D, \y[1][\s'] \vdash e[e'/x] : \vp$ \` by induction hypothesis (2,3)\\
  (5) $\G; \D \vdash \lambda\y[1][\s'].~e[e'/x] : \s' \to_1\vp$ \` by $\lambda I_1$\\
  (6) $(\lambda \y[\pi][\s'].~e)[e'/x] = (\lambda \y[\pi][\s'].~e[e'/x])$ \` by def. of subst.\\
\end{tabbing}

\item[Case:] $\lambda I_\omega$
\begin{tabbing}
  (1) $\G, \xo; \D \vdash \lambda\y[\omega][\s'].~e : \s'\to_\omega\vp$\\
  (2) $\G; \cdot \vdash e' : \sigma$\\
  (3) $\G, \xo, \y[\omega][\s']; \D \vdash e : \vp$ \` by inversion on $\lambda I_\omega$\\
  (4) $\G, \y[\omega][\s']; \D, \vdash e[e'/x] : \vp$ \` by induction hypothesis (2,3)\\
  (5) $\G; \D \vdash \lambda\y[\omega][\s'].~e[e'/x] : \s' \to_\omega\vp$ \` by $\lambda I_\omega$\\
  (6) $(\lambda \y[\pi][\s'].~e)[e'/x] = (\lambda \y[\pi][\s'].~e[e'/x])$ \` by def. of subst.\\
\end{tabbing}

\item[Case:] $Var_\omega$
\begin{tabbing}
  (1) $\G, x{:}_\omega; \cdot \sigma \vdash x : \sigma$\\
  (2) $\G; \cdot \vdash e' : \s$\\
  (4) $x[e'/x] = e'$ \` by def. of substitution\\
  (5) $\G; \cdot \vdash e' : \sigma$ \` by (2)\\
  % (6) $\G, \G' \vdash e' : \sigma$ \` by $Weaken_\omega$ (3)\\
\end{tabbing}

\item[Case:] $Var_\omega$
\begin{tabbing}
  (1) $\G, \xo; \cdot \vdash y : \vp$\\
  (2) $\G; \cdot \vdash e' : \s$\\
  (3) $y[e'/x] = y$ \` by def. of substitution\\
  (4) $\G; \cdot \vdash y : \vp$ \` by inversion on $Weaken_\omega$ (1)\\
\end{tabbing}

\item[Case:] $Var_1$
\begin{tabbing}
  (1) Impossible. The context in $Var_1$ is empty.
\end{tabbing}

\item[Case:] $Var_\Delta$
\begin{tabbing}
  (1) Impossible. The context in $Var_\Delta$ only contains linear variables.
\end{tabbing}

\item[Case:] $Split$
\begin{tabbing}
    TODO
\end{tabbing}

\item[Case:] $\lambda E_{1,p}$
\begin{tabbing}
  (1) $\G, \xo; \D,\D' \vdash e~e'' : \vp$\\
  (2) $\G; \cdot \vdash e' : \s$\\
  % (3) $\G, \xo, \xo, \G'' \vdash e~e'' : \vp$ \` by $Contract_\omega$\\
  (3) $\G, \xo; \D \vdash e : \s'\to_{1,p}\vp$ \` by inversion on $\lambda E_{1,p}$\\
  (4) $\G, \xo; \D' \vdash e'' : \s'$ \` by inversion on $\lambda E_{1,p}$\\
  (5) $\G; \D \vdash e[e'/x] : \s'\to_{1,p}\vp$ \` by induction hypothesis (2,3)\\
  (6) $\G; \D' \vdash e''[e'/x] : \s'$ \` by induction hypothesis (2,4)\\
  (7) $\G; \D, \D' \vdash e[e'/x]~e''[e'/x] : \vp$ \` by $\lambda E_{1,p}$ (5,6)\\
  % (9) $\G, \G'', \G' \vdash e[e'/x]~e''[e'/x] : \vp$ \` by $Contract_\omega$ (3)\\
  (8) $(e~e'')[e'/x] = (e[e'/x]~e''[e'/x])$ \` by def. of subst.\\
\end{tabbing}

\item[Case:] $\lambda E_\omega$
\begin{tabbing}
    (1) $\G, \xo; \D \vdash e~e'' : \vp$\\
    (2) $\G; \cdot \vdash e' : \s$\\
    (3) $\G, \xo; \D \vdash e : \s'\to_\omega\vp$ \` by inversion on $\lambda E_\omega$\\
    (4) $\G, \xo; \cdot \vdash e'' : \s'$ \` by inversion on $\lambda E_\omega$\\
    (5) $\G; \D \vdash e[e'/x] : \s'\to_1\vp$ \` by induction hypothesis (2,3)\\
    (6) $\G; \cdot \vdash e''[e'/x] : \s'$ \` by induction hypothesis (2,4)\\
    (7) $\G; \D \vdash e[e'/x]~e''[e'/x] : \vp$ \` by $\lambda E_\omega$ (5,6)\\
    (8) $(e~e'')[e'/x] = (e[e'/x]~e''[e'/x])$ \` by def. of subst.\\
\end{tabbing}

\item[Case:] $Let$
\begin{tabbing}
    (1) $\G, \xo; \D, \D' \vdash \llet{\yD = e}{e''} : \vp$\\
    (2) $\G; \cdot \vdash e' : \sigma$\\
    (3) $\G,\xo,\yD; \D, \D' \vdash e'' \vp$ \` by inversion on $Let$\\
    (4) $\G,\xo; \D \vdash e : \s'$ \` by inversion on $Let$\\
    (5) $\G,\yD; \D \vdash e''[e'/x] : \vp$ \` by induction hypothesis (2,3)\\
    (6) $\G; \D \vdash e[e'/x] : \s'$ \` by induction hypothesis (2,4)\\
    (7) $\G;\D,\D' \vdash \llet{\yD = e[e'/x]}{e''[e'/x]}$ \` by $Let$ (5,6)\\
    (8) $(\llet{\yD = e}{e''})[e'/x] = (\llet{\yD = e[e'/x]}{e''[e'/x]})$
\end{tabbing}

\item[Case:] $LetRec$
\begin{tabbing}
    (1) $\G, \xo; \D, \D' \vdash \lletrec{\ov{\yD = e}}{e''} : \vp$\\
    (2) $\G'; \cdot \vdash e' : \sigma$\\
    (3) $\G,\xo,\ov{\yD}; \D, \D' \vdash e'' : \vp$ \` by inversion on $LetRec$\\
    (4) $\ov{\G,\xo, \ov{\yD}; \D \vdash e : \s'}$ \` by inversion on $LetRec$\\
    (5) $\G, \ov{\yD}; \D, \D' \vdash e''[e'/x] : \vp$ \` by induction hypothesis (2,3)\\
    (6) $\ov{\G,\ov{\yD}; \D \vdash e[e'/x] : \s'}$ \` by induction hypothesis (2,4)\\
    (7) $\G; \D, \D' \vdash \lletrec{\ov{\yD = e[e'/x]}}{e''[e'/x]} : \vp$ \` by $LetRec$ (5,6)\\
    (8) $(\lletrec{\ov{\yD = e}}{e''})[e'/x] = (\lletrec{\ov{\yD = e[e'/x]}}{e''[e'/x]})$
\end{tabbing}

\item[Case:] $CaseWHNF$
\begin{tabbing}
    (1) TODO
\end{tabbing}

\item[Case:] $CaseNotWHNF$
\begin{tabbing}
    (1) TODO
\end{tabbing}

\end{description}

\end{proof}

\begin{sublemma}[Substitution of unrestricted variables on case alternatives
    preserves typing]
\emph{If $\G, \xo \vdash_{alt} \rho \to e :_\Delta \s \Rightarrow \vp$ and $\G' \vdash e' : \s$ and
    $\hasnolinearvars{\G'}$ then $\G, \G' \vdash_{alt} \rho \to e[e'/x] :_\Delta \s \Rightarrow \vp$}
\end{sublemma}

\begin{proof}
By structural induction on the $alt$ judgment.

\begin{description}
\item[Case:] $AltN$
\begin{tabbing}
    TODO
\end{tabbing}

\item[Case:] $Alt0$
\begin{tabbing}
    TODO
\end{tabbing}

\item[Case:] $Alt_\_$
\begin{tabbing}
    TODO
\end{tabbing}

\end{description}
\end{proof}
