\begin{lemma}[Substitution of linear variables preserves typing]
  If $\judg[\G][\D,\xl][\d]{e}{\vp}$ and $\judg[\G][\D'][\d']{e}{\s}$
  then $\judg[\G][\D,\D'][\subst{\d}{\D'}{x}, \d']{e[e'/x]}{\vp}$,
  where $\d[\D'/x]$ substitutes all occurrences of $x$ in the usage
  environments of variables in $\d$ by the linear variables in $\D'$.
  (really, $x$ couldn't appear anywhere else since $x$ is linear).
\end{lemma}

% TODO: Short paragraph about the proof for case alternatives sublemma for
% Alt_0: It's hard because one must consider two different subcases, one in
% which $x$ is part of the scrutinee and other in which it isn't, to prove the goal...

% Template:
% (2) $\judg[][][]{}{}$\\

\begin{proof}
By structural induction on the first derivation.

\begin{description}

\item[Case:] $\Lambda I$
\begin{tabbing}
  (1) $\Gamma; \D, x{:}_1\sigma; \d \vdash \Lambda p.~e : \forall p.~\varphi$\\
  (2) $\G; \D'; \d' \vdash e' : \sigma$\\
  (3) $\G, p; \D,x{:}_1\sigma; \d \vdash e : \varphi$ \` by inversion on $\Lambda I$\\
  (4) $p \notin \Gamma$ \` by inversion on $\Lambda I$\\
  (5) $\G,p; \D,\D'; \d[\D'/x], \d' \vdash e[e'/x] : \varphi$ \` by induction hypothesis by (2,3)\\
  (6) $\G;\D,\D';\d[\D'/x], \d' \vdash \Lambda p.~e[e'/x] : \forall p.~\varphi$ \` by $\Lambda I$ (4,5)\\
  (7) $(\Lambda p.~e)[e'/x] = (\Lambda p.~e[e'/x])$ \` by def. of substitution\\
\end{tabbing}

\item[Case:] $\Lambda E$
\begin{tabbing}
  (1) $\Gamma; \D, x{:}_1\sigma; \d \vdash e~\pi: \varphi[\pi/p]$\\
  (2) $\G; \D'; \d' \vdash e' : \sigma$\\
  (3) $\G; \D, \xl; \d' \vdash e : \forall p.~\varphi$ \` by inversion on $\Lambda E$\\
  (4) $\G \vdash_{mult} \pi$ \` by inversion on $\Lambda E$\\
  (5) $\G; \D,\D';\d[\D'/x],\d' \vdash e[e'/x] : \forall p.~\varphi$ \` by induction hypothesis by (2,3)\\
  (6) $\G; \D,\D';\d[\D'/x], \d' \vdash e[e'/x]~\pi : \varphi[\pi/p]$ \` by $\Lambda E$ (4,5)\\
  (7) $(e~\pi)[e'/x] = e[e'/x] \pi$ \` by def. of substitution\\
\end{tabbing}

\item[Case:] $\lambda I_1$
\begin{tabbing}
  (1) $\G; \D, \xl; \d \vdash \lambda y{:}_1\sigma'.~e : \sigma' \to_1 \varphi$\\
  (2) $\G; \D'; \d' \vdash e' : \sigma$\\
  (3) $\G; \D, \xl, y{:}_1\sigma'; \d' \vdash e : \varphi$ \` by inversion on $\lambda I$\\
  (4) $\G; \D, y{:}_1\sigma', \D'; \d[\D'/x], \d' \vdash e[e'/x] : \varphi$ \` by induction hypothesis by (2,3)\\
  (5) $\G; \D,\D'; \d[\D'/x],\d' \vdash \lambda y{:}_1\sigma'.~e[e'/x] : \sigma' \to_1 \varphi$ \` by $\lambda I$ (4)\\
  (6) $(\lambda y{:}_1\sigma'.~e)[e'/x] = (\lambda y{:}_1\sigma'.~e[e'/x])$ \` by def. of substitution\\
\end{tabbing}

\item[Case:] $\lambda I_\omega$
\begin{tabbing}
  (1) $\G; \D, \xl; \d \vdash \lambda y{:}_\omega\sigma'.~e : \sigma' \to_\omega \varphi$\\
  (2) $\G; \D'; \d' \vdash e' : \sigma$\\
  (3) $\G, y{:}_\omega\sigma'; \D, \xl; \d' \vdash e : \varphi$ \` by inversion on $\lambda I$\\
  (4) $\G, y{:}_\omega\sigma'; \D, \D'; \d[\D'/x], \d' \vdash e[e'/x] : \varphi$ \` by induction hypothesis by (2,3)\\
  (5) $\G; \D,\D'; \d[\D'/x],\d' \vdash \lambda y{:}_\omega\sigma'.~e[e'/x] : \sigma' \to_1 \varphi$ \` by $\lambda I$ (4)\\
  (6) $(\lambda y{:}_\omega\sigma'.~e)[e'/x] = (\lambda y{:}_\omega\sigma'.~e[e'/x])$ \` by def. of substitution\\
\end{tabbing}

\item[Case:] $Var_1$
\begin{tabbing}
  (1) $\G;x{:}_1\sigma;\d \vdash x : \sigma$\\
  (2) $\G;\D';\d' \vdash e' : \sigma$\\
  (3) $x[e'/x] = e'$ \` by def. of substitution\\
  % (3) $\cdot[\lin{\G'}/x] = \cdot$ \` by def. of substitution\\
    (4) $\G;\D';\d,\d' \vdash e' : \sigma$ \` by (2)\\ % TODO: And weaken?
\end{tabbing}

\item[Case:] $Var_\omega$\\
  (1) Impossible. $x{:}_1\sigma$ can't be in the context.\\

\item[Case:] $Var_\Delta$
\begin{tabbing}
  (1) $\D, x{:}_1\sigma, y{:}_{\Delta,\xl}\varphi \vdash y : \varphi$\\
  (2) $\G' \vdash e' : \sigma$\\
  (3) $y[e'/x] = y$\\
  (4) $\D, \xl, \y[\Delta,\xl][\vp] \vdash y : \vp$\\
  Subcase $\G'$ has linear variables\\
  (5) Impossible. $\y[\Delta][\s]$ is only well typed if the context is exactly $\Delta,\y[\D][\s]$\\
  Subcase $\G'$ has no linear variables\\
  (5) $\G', \D, \xl, \y[\Delta,\xl][\vp] \vdash y : \vp$ \` by $Weaken_\omega$\\

\end{tabbing}

\item[Case:] $\lambda E_1$
\begin{tabbing}
  (1) $\G, \xl, \G'' \vdash e~e'' : \vp$\\
  (2) $\G' \vdash e' : \s$\\
  Subcase $x$ occurs in $e$\\
  (3) $\G, \xl \vdash e : \s' \to_1 \vp$\` by inversion on $\lambda E_1$\\
  (4) $\G'' \vdash e'' : \s'$\` by inversion on $\lambda E_1$\\
  (5) $\G[\lin{\G'}/x], \G' \vdash e[e'/x] : \s' \to_1 \vp$\` by induction hypothesis (2,3)\\
  (6) $\G[\lin{\G'}/x], \G', \G'' \vdash e[e'/x]~e'' : \vp$\` by $\lambda E_1$\\
  (7) $\G''[\lin{\G'}/x] = \G''$\` $x$ doesn't occur in $e''$, so $\Delta$-bound vars in $e''$ \\
      \` couldn't contain $x$ and still be well-typed.\\
  (8) $(e[e'/x]~e'') = (e~e'')[e'/x]$ \` because $x$ does not occur in $e''$\\
  Subcase $x$ occurs in $e''$\\
  (3) $\G \vdash e : \s' \to_1 \vp$\` by inversion on $\lambda E_1$\\
  (4) $\G'', \xl \vdash e'' : \s'$\` by inversion on $\lambda E_1$\\
  (5) $\G''[\lin{\G'}/x], \G' \vdash e''[e'/x] : \s'$\` by induction hypothesis (2,4)\\
  (6) $\G, \G''[\lin{\G'}/x], \G' \vdash e~e''[e'/x] : \vp$\` by $\lambda E_1$\\
  (7) $\G[\lin{\G'}/x] = \G$\` $x$ doesn't occur in $e$, so $\Delta$-bound vars in $e$ \\
      \` couldn't contain $x$ and still be well-typed.\\
  (8) $(e~e''[e'/x]) = (e~e'')[e'/x]$ \` because $x$ does not occur in $e$\\
\end{tabbing}

\item[Case:] $\lambda E_\omega$
\begin{tabbing}
  (1) $\G, \xl, \G'' \vdash e~e'' : \vp$\\
  (2) $\G' \vdash e' : \s$\\
  (3) $\hasnolinearvars{\G'}$\\
  (4) $x$ does not occur in $e''$\` by (3)\\
  (5) $\G, \xl \vdash e : \s' \to_\omega \vp$\` by inversion on $\lambda E_\omega$\\
  (6) $\G'' \vdash e'' : \s'$\` by inversion on $\lambda E_\omega$\\
  (7) $\G[\lin{\G'}/x], \G' \vdash e[e'/x] : \s' \to_\omega \vp$\` by induction hypothesis (2,3,5)\\
  (6) $\G[\lin{\G'}/x], \G', \G'' \vdash e[e'/x]~e'' : \vp$\` by $\lambda E_\omega$\\
  (7) $\G''[\lin{\G'}/x] = \G''$\` $x$ doesn't occur in $e''$, so $\Delta$-bound vars in $e''$ \\
      \` couldn't contain $x$ and still be well-typed.\\
  (8) $(e[e'/x]~e'') = (e~e'')[e'/x]$ \` because $x$ does not occur in $e''$\\
\end{tabbing}

\item[Case:] $Let$
\begin{tabbing}
  (1) $\G' \vdash e' : \s$\\
  (2) $\hasnolinearvars{\G''}$\\
  Subcase $x$ occurs in $e$\\
  (3) $\G, \G'', \D, \xl \vdash \llet{\y[\D,\xl][\s'] = e}{e''} : \vp$\\
  (4) $\G, \D, \xl, \y[\D,\xl][\s'] \vdash e'' : vp$\` by inversion on $Let$\\
  (5) $\G'', \D, \xl \vdash e : \s'$\` by inversion on $Let$\\
  (6) $\G[\lin{\G'}/x], \D, \y[\D,\lin{\G'}][\s'], \lin{\G'}, \unr{\G'} \vdash
  e''[e'/x]$\` by induction hypothesis $(1,4)$\\
  (7) $\G''[\lin{\G'}/x], \D, \lin{\G'}, \unr{\G'} \vdash e[e'/x] : \s'$ \` by induction hypothesis $(1,5)$\\
  (8) $\hasnolinearvars{\G''[\lin{\G'}/x]}$\` by (2) and def. of env. subst.\\
  (9) $\G[\lin{\G'}/x], \G''[\lin{\G'}/x], \D, \lin{\G'}, \unr{\G'}, \unr{\G'}
  \vdash \llet{\y[\D,\lin{\G'}][\s'] = e[e'/x]}{e''[e'/x]} : \vp$ \` (6,7,8)\\ % by $Let$ %
  (10) $(\G, \G'')[\lin{\G'}/x], \D, \lin{\G'}, \unr{\G'} \vdash
  \llet{\y[\D,\lin{\G'}][\s'] = e[e'/x]}{e''[e'/x]} : \vp$ \` by $Contract_\omega$\\
  (11) $\Delta[\lin{\G'}/x] = \Delta$ \` $\Delta$ only has linear vars, by construction\\
  (12) $(\llet{\y[\D,\lin{\G'}][\s'] = e[e'/x]}{e''[e'/x]}) =
  (\llet{\y[\D,\lin{\G'}][\s'] = e}{e''})[e'/x]$ \` by subst.\\
  Subcase $x$ does not occur in $e$\\
  (3) $\G, \xl, \G'', \D \vdash \llet{\yD = e}{e''} : \vp$\\
  (4) $\G, \xl, \D, \yD \vdash e'' : \vp$ \` by inversion on $Let$\\
  (5) $\G'', \D \vdash e : \s'$ \` by inversion on $Let$\\
  (6) $\G[\lin{\G'}/x], \D, \yD, \G' \vdash e''[e'/x] : \vp$\` by induction hypothesis (1,4)\\
  (7) $\G[\lin{\G'}/x], \G'', \D, \G' \vdash \llet{\yD = e}{e''[e'/x]} : \vp$ \`
  by $Let$ (2,5,6)\\
  (8) $\D[\lin{\G'}/x] = \D$\` $\Delta$ only has linear vars, by
  construction\\
  (9) $\G''[\lin{\G'}/x] = \G''$\` by (2) and $x \notin \Delta$ in this
  subcase,\\
  \` $\G''$ can't have a $\Delta$-bound var mentioning $x$.\\
  (10) $\llet{\yD = e}{e''[e'/x]} = (\llet{\yD = e}{e''})[e'/x]$\` by $x$ does
  not occur in $e$\\
\end{tabbing}

\item[Case:] $LetRec$
\begin{tabbing}
  (1) $\G' \vdash e' : \s$\\
  (2) $\ov{\hasnolinearvars{\G''_i}}$\` by inversion on $LetRec$\\
  Subcase $\xl$ occurs in some $e_i$\\
  (3) $\G, \ov{\G''_i}, \D, \xl \vdash \lletrec{\ov{\var[y_i][\D,\xl][\s_i] = e_i}}{e''} : \vp$\\
  (4) $\G, \ov{\var[y_i][\D,\xl][\s_i]}, \D, \xl \vdash e'' : \vp$\` by inversion on $LetRec$\\
  (5) $\ov{\G''_i, \D, \xl, \ov{\var[y_i][\D, \xl][\s_i]}, \vdash e_i : \s_i}$\` by inversion on $LetRec$\\
  (6) $\G[\G'_1/x], \ov{\var[y_i][\D, \G'_1][\s_i]}, \G', \D \vdash e''[e'/x] : \vp$ \` by induction hypothesis (1,4)\\
  (7) $\ov{\G''_i, \D, \ov{\var[y_i][\D, \G'_1][\s_i]} \vdash e_i[e'/x] : \s_i}$\` by induction hypothesis (1,5)\\
  (8) $\G[\G'_1/x], \ov{\G''_i}, \G', \D \vdash \lletrec{\ov{\var[y_i][\D,\G'_1][\s_i] = e_i[e'/x]}}{e''[e'/x]} : \vp$\` by $LetRec$\\
  (9) $(\lletrec{\ov{\var[y_i][\D,\G'_1][\s_i] = e_i}}{e''})[e'/x] = \lletrec{\ov{\var[y_i][\D,\G'_1][\s_i] = e_i[e'/x]}}{e''[e'/x]}$\\
  Subcase $\xl$ does not occur in any $e_i$\\
  (3) $\G, \xl, \ov{\G''_i}, \D \vdash \lletrec{\ov{\var[y_i][\D][\s_i] = e_i}}{e''} : \vp$\\
  (4) $\G, \xl, \ov{\var[y_i][\D][\s_i]}, \D \vdash e'' : \vp$\` by inversion on $LetRec$\\
  (5) $\ov{\G''_i, \D, \ov{\var[y_i][\D][\s_i]}, \vdash e_i : \s_i}$\` by inversion on $LetRec$\\
  (6) $\G[\G'_1/x], \ov{\var[y_i][\D][\s_i]}, \D \vdash e''[e'/x] : \vp$\` by i.h. (1,4)\\
  (7) $\G[\G'_1/x], \ov{\G''_i}, \D, \G' \vdash \lletrec{\ov{\var[y_i][\D][\s_i] = e_i}}{e''[e'/x]} : \vp$\` by $LetRec$\\
  (8) $\lletrec{\ov{\var[y_i][\D][\s_i] = e_i}}{e''[e'/x]} =
  (\lletrec{\ov{\var[y_i][\D][\s_i] = e_i}}{e''})[e'/x]$\` by subcase\\
\end{tabbing}

\item[Case:] $CaseWHNF$
\begin{tabbing}
  (1) $\judg[\G][\D'][\d']{e'}{\s}$\\
  Subcase $x$ occurs in $e$\\
  (2) $\judg[\G][\D,\xl,\D''][\d]{\ccase{e}{\z[\D,\xl][\s']~\{\ov{\rho\to e''}\}}}{\vp}$\\
  (3) $e$ is in WHNF\\
  (4) $\judg[\G][\D,\xl][\d]{e}{\s'}$\\
  (5) $\ov{\judg[\G][\D,\xl,\D''][\d,\zr{\D,\xl}{\s'}]{\rho\to e''}{\s' \Longrightarrow \vp}[alt][\D,\xl]}$\\
  (6) $\judg[\G][\D,\D'][\subst{\d}{\D'}{x}, \d']{e[e'/x]}{\vp}$\`by i.h.\\
  (7) $\ov{\judg[\G][\D,\D',\D''][\subst{\d}{\D'}{x},\zr{\D,\D'}{\s'}]{\rho\to e''[e'/x]}{\s' \Longrightarrow \vp}[alt][\D,\D']}$\` by i.h.\\
  (8) $\judg[\G][\D,\D',\D''][\subst{\d}{\D'}{x},\d']{\ccase{e[e'/x]}{\z[\D,\D'][\s']~\{\ov{\rho\to e''[e'/x]}\}}}{\vp}$\\
  Subcase $x$ occurs in $\ov{e''}$\\
  (2) $\judg[\G][\D,\D'',\xl][\d]{\ccase{e}{\z[\D][\s']~\{\ov{\rho\to e''}\}}}{\vp}$\\
  (3) $e$ is in WHNF\\
  (4) $\judg[\G][\D][\d]{e}{\s'}$\\
  (5) $\ov{\judg[\G][\D,\D'',\xl][\d,\zr{\D}{\s'}]{\rho\to e''}{\s' \Longrightarrow \vp}[alt][\D]}$\\
  (6) $e[e'/x] = e, \d[\D'/x]=\d$\` by $x$ does not occur in $e$\\
  (7) $\ov{\judg[\G][\D,\D'',\D'][\subst{\d}{\D'}{x},\zr{\D}{\s'}]{\rho\to e''[e'/x]}{\s' \Longrightarrow \vp}[alt][\D]}$\`by i.h.\\
  (8) $\judg[\G][\D,\D'',\D'][\subst{\d}{\D'}{x},\d']{\ccase{e}{\z[\D][\s']~\{\ov{\rho\to e''[e'/x]}\}}}{\vp}$\\
\end{tabbing}

\item[Case:] $CaseNotWHNF$
\begin{tabbing}
  (1) $\judg[\G][\D'][\d']{e'}{\s}$\\
  Subcase $x$ occurs in $e$\\
    (2) $\judg[\G][\D,\xl,\D''][\d,\d'']{\ccase{e}{\z[\irr{\D,\xl}][\s']~\{\ov{\rho\to e''}\}}}{\vp}$\\
    (3) $e$ is definitely not in WHNF\\
    (4) $\judg[\G][\D,\xl][\d]{e}{\s'}$\`by inv.\\
    (5) $\ov{\judg[\G][\irr{\D,\xl},\D''][\irr{\d},\d'',\zr{\irr{\D,\xl}}{\s'}]{\rho\to e''}{\s' \Longrightarrow \vp}[alt][\irr{\D,\xl}]}$\`by inv.\\
    (6) $\judg[\G][\D,\D'][\subst{\d}{\D'}{x}, \d']{e[e'/x]}{\vp}$\`by i.h.\\
    (7) $\ov{\judg[\G][\irr{\D,\D'},\D''][\d'',\subst{\irr{\d}}{\irr{\D'}}{\irr{x}},\zr{\D,\D'}{\s'}]{\rho\to e''[e'/x]}{\s' \Longrightarrow \vp}[alt][\D,\D']}$\` by subst. of p. irr. vars in alt.\\
    (8) $\judg[\G][\D,\D',\D''][\subst{(\d,\d'')}{\D'}{x},\d']{\ccase{e[e'/x]}{\z[\D,\D'][\s']~\{\ov{\rho\to e''[e'/x]}\}}}{\vp}$\\
  Subcase $x$ occurs in $\ov{e''}$\\
    (2) $\judg[\G][\D,\D'',\xl][\d,\d'']{\ccase{e}{\z[\irr{\D}][\s']~\{\ov{\rho\to e''}\}}}{\vp}$\\
    (3) $e$ is definitely not in WHNF\\
    (4) $\judg[\G][\D][\d]{e}{\s'}$\\
    (5) $\ov{\judg[\G][\D,\D'',\xl][\d,\d'',\zr{\D}{\s'}]{\rho\to e''}{\s' \Longrightarrow \vp}[alt][\D]}$\\
    (6) $e[e'/x] = e, \d[\D'/x]=\d$\` by $x$ does not occur in $e$\\
    (7) $\ov{\judg[\G][\D,\D'',\D'][\d,\subst{\d''}{\D'}{x},\zr{\D}{\s'}]{\rho\to e''[e'/x]}{\s' \Longrightarrow \vp}[alt][\D]}$\`by i.h.\\
    (8) $\judg[\G][\D,\D'',\D'][\d,\subst{\d''}{\D'}{x},\d']{\ccase{e}{\z[\D][\s']~\{\ov{\rho\to e''[e'/x]}\}}}{\vp}$\\
\end{tabbing}

\item[Case:] $CaseVar$
\begin{tabbing}
    Great! Substitution doesn't preserve types for this case...
\end{tabbing}


\end{description}
\end{proof}

\begin{sublemma}[Substitution of linear variables on case alternatives
    preserves typing]
  If $\judg[\G][\D,\xl][\d]{\rho\to e}{\s \Longrightarrow \vp}[alt][\D_s]$ and
    $\judg[\G][\D'][\d']{e'}{\s}$ then
    $\judg[\G][\D,\D'][\subst{\d}{\D'}{x},\d']{\rho \to e[e'/x]}{\s \Longrightarrow \vp}[alt][\subst{\D_s}{\D'}{x}]$
\end{sublemma}

\begin{proof}
By structural induction on the $alt$ judgment.

\begin{description}
\item[Case:] $AltN$
\begin{tabbing}
  (1) $\judg[\G'][\D'][\d']{e'}{\s}$\\
  (2) $\judg[\G][\D,\xl][\d]{\konstructor~\to e}{\s' \Longrightarrow \vp}[alt][\D_s]$\\
  (3) $n > 0$\\
  (4) $\judg[\G,\ov{\xo}][\D,\xl][\d,\ov{y_i{:}_{\lctag{\D_s}{K_i}}\s_i}]{e}{\vp}$\\
  (5) $\judg[\G,\ov{\xo}, \G'][\D,\D'][\subst{\d}{\D'}{x},\ov{y_i{:}_{\lctag{\subst{\D_s}{\D'}{x}}{K_i}}\s_i},\d']{e[e'/x]}{\vp}$\\
  (6) $\judg[\G,\G'][\D,\D'][\subst{\d}{\D'}{x},\d']{\rho \to e[e'/x]}{\s' \Longrightarrow \vp}[alt][\subst{\D_s}{\D'}{x}]$\\
\end{tabbing}

\item[Case:] $Alt0$
    This is one of the most interesting proof cases, and particularly hard to prove.
        \begin{itemize}
            \item The first insight is to divide the proof into two subcases, accounting
                for when the scrutinee (and hence $\D_s$) contains the linear resource and when it does not.
            \item The second insight is to recall that $\D$ and $\D'$ are
                disjoint to be able to prove the subcase in which $x$ does not
                occur in the scrutinee
            \item The third insight is to \emph{create} linear resources
                seemingly out of nowhere \emph{under a substitution that
                removes them}. We see this happen in the case where $x$ occurs
                in the scrutinee, for both the linear and affine contexts (see 5 and 6).
        \end{itemize}
        TODO: Validate the two TODOs in the source
\begin{tabbing}
  (1) $\judg[\G][\D'][\d']{e'}{\s}$\\
  Subcase $x$ occurs in scrutinee\\
    (2) $\judg[\G][\D,\xl][\d]{K~\ov{\xo}~\to e}{\s' \Longrightarrow \vp}[alt][\D_s,\xl]$\\
    (2.5) $\judg[\G,\ov{\xo}][\subst{(\D,\xl)}{\cdot}{\D_s,x}][\subst{\d}{\cdot}{\D_s,x}]{e}{\vp}$\`by inv.\\
    (3) $\judg[\G,\ov{\xo}][\subst{\D}{\cdot}{\D_s}][\subst{\d}{\cdot}{\D_s,x}]{e}{\vp}$\\
    (4) $e[e'/x] = e$\` since $x$ cannot occur in $e$ (erased from cx)\\
    (5) $\D[\cdot/\D_s] = (\D,\D')[\cdot/\D_s,\D']$\`by def. of subst.\\
    (6) $\d[\cdot/\D_s,x] = \d[\D'/x][\cdot/\D_s,\D']$\` by def. of subst.\\
    (7) $\judg[\G,\ov{\xo}][\subst{(\D,\D')}{\cdot}{\D_s,\D'}][\subst{\subst{\d}{\D'}{x}}{\cdot}{\D_s,\D'}]{e[e'x]}{\vp}$\` by (4,5,6)\\
    (8) $\judg[\G,\ov{\xo}][\subst{(\D,\D')}{\cdot}{\D_s,\D'}][\subst{\subst{\d}{\D'}{x},\d'}{\cdot}{\D_s,\D'}]{e[e'x]}{\vp}$\` by $Weaken_\Delta$\\ % (TODO: POSSO?)
    (9) $\judg[\G][\D,\D'][\subst{\d}{\D'}{x},\d']{K~\ov{\xo}~\to e[e'/x]}{\s' \Longrightarrow \vp}[alt][\D_s,\D']$\\
  Subcase $x$ does not occur in scrutinee\\
    (2) $\judg[\G][\D,\xl][\d]{K~\ov{\xo}~\to e}{\s' \Longrightarrow \vp}[alt][\D_s]$\\
    (3) $\judg[\G,\ov{\xo}][\subst{\D}{\cdot}{\D_s},\xl][\subst{\d}{\cdot}{\D_s}]{e}{\vp}$\`by $x$ does not occur in $\D_s$\\
    (4) $\judg[\G,\ov{\xo}][\subst{\D}{\cdot}{\D_s},\D'][\subst{\d}{\cdot}{\D_s},\d']{e[e'/x]}{\vp}$\`by i.h.\\
    (5) $\judg[\G,\ov{\xo}][\subst{(\D,\D')}{\cdot}{\D_s}][\subst{(\d,\d')}{\cdot}{\D_s}]{e[e'/x]}{\vp}$\\
    \`by $\D$ and $\D'$ and $\d$ and $\d'$ being disjoint by hypothesis,\\
    \`and $\D_s$ being a subset of $\D$\\ % (TODO CHECK)\\
    \`so $\D_s$ can't occur in $\d'$ either\\
    (6) $\D_s[\D'/x] = \D_s$\`by $x$ does not occur in $\D_s$\\
    (7) $\judg[\G][\D,\D'][\d,\d']{K~\ov{\xo}~\to e[e'/x]}{\s' \Longrightarrow \vp}[alt][\subst{\D_s}{\D'}{x}]$\\
\end{tabbing}

\item[Case:] $Alt\_$ (Trivial induction)
\begin{tabbing}
    (1) $\judg[\G][\D'][\d']{e'}{\s}$\\
    (2) $\judg[\G][\D,\xl][\d]{\_~\to e}{\s' \Longrightarrow \vp}[alt][\D_s]$\\
    (3) $\judg[\G][\D,\xl][\d]{e}{\vp}$\\
    (4) $\judg[\G][\D,\D'][\subst{\d}{\D'}{x},\d']{e[e'/x]}{\vp}$\\
    (5) $\judg[\G][\D,\D'][\subst{\d}{\D'}{x},\d']{\_~\to e[e'/x]}{\s' \Longrightarrow \vp}[alt][\D_s,\D']$\\
\end{tabbing}

\end{description}

\end{proof}

