
{-
If
  Γ,Δ,xΔσ |- e : \vp
  Γ' |- e' : σ
Then
  Γ,Γ' |- e[e'/x] : \vp
-}



\z y ->
  let x_{z,y} = (z,y)
   in e

Subcase x occurs in e
z,y,x_{z,y} |- e
z,y |- (z,y)
z,y |- e[(z,y)/x]


\x y ->
  case K x y of z
    K x1 x2 -> e

Subcase z occurs in e
x,y |- K x y
x1,x2,z |- e
x,y|-e[K x y/e]

Subcase x1,x2 occurs in e



-----------

let x = e in e1 ==> let x = e in e1[e/x]


If 
  Γ |- let x = e in e1 : T
Then
  Γ |- let x = e in e1[e/x] : T

Proof
  (1) Γ |- let x = e in e1 : T
  (2) Γ |- let x = e in e1 : T by inv
  (3) by subst
  (4) ...


